@prefix : <urn:ontoinsights:dna:> .
@prefix dna: <urn:ontoinsights:dna:> .
@prefix owl: <http://www.w3.org/2002/07/owl#> .
@prefix rdf: <http://www.w3.org/1999/02/22-rdf-syntax-ns#> .
@prefix rdfs: <http://www.w3.org/2000/01/rdf-schema#> .
@prefix xsd: <http://www.w3.org/2001/XMLSchema#> .

########################################################################
# File defining semantics related to participants/actors/agents in events 
# and states/situations
# 
# Created: February 9 2020
# Last modified: October 31 2023
# 
# Licensed by OntoInsights, LLC
# Creative Commons Attribution 4.0 International (CC BY 4.0)
# 
# Unless required by applicable law or agreed to in writing,
# software distributed under the License is distributed on an
# "AS IS" BASIS, WITHOUT WARRANTIES OR CONDITIONS OF ANY KIND,
# either express or implied.
# 
# Changes:
#  Reset change history and simplified
########################################################################


########################################################################
# Classes
########################################################################

:ArmedForce a owl:Class ;
  rdfs:subClassOf :GovernmentalEntity ;
  rdfs:label "Armed Force"@en ;
  rdfs:comment "A GPE's military force."@en ;
  :wordnet_noun_synset "08215965", "08207684" .

:Business a owl:Class ;
  rdfs:subClassOf :OrganizationalEntity ;
  rdfs:label "Corporation"@en ;
  rdfs:comment "A business/company that is legally recognized and acts as a single entity."@en ;
  :wordnet_noun_synset "08076248" .

:DisplacedPerson a owl:Class ;
  rdfs:subClassOf :Person ;
  rdfs:label "Displaced Person or Refugee"@en ;
  rdfs:comment "A Person or Group who is forced to leave their home due to violence, natural disasters, war, persecution, etc."@en ;
  :wordnet_noun_synset "10037615", "10535609" .

:EthnicGroup a owl:Class ;
  rdfs:subClassOf :GroupOfAgents ;
  rdfs:label "Ethnic Group"@en ;
  rdfs:comment "An EthnicGroup is a sett of persons who identify based on ethnicity - e.g., having a common genealogy, ancestry, language, history, culture, nation, ...'."@en ;
  :wordnet_noun_synset "04806382" .

:ExecutiveAndLegislativeGroup a owl:Class ;
  rdfs:subClassOf :GovernmentalEntity ;
  rdfs:label "Executive and Legislative Group"@en ;
  rdfs:comment "A type of GovernmentalEntity responsible for legislation (such as the US Congress) and for enforcing those laws and governing."@en .

:FaithBasedOrganization a owl:Class ;
  rdfs:subClassOf :OrganizationalEntity ;
  rdfs:label "Faith-Based Organization"@en ;
  rdfs:comment "An organization that provides infrastructure and services to a religious/faith-based community."@en .

:GovernmentalEntity a owl:Class ;
  rdfs:subClassOf :OrganizationalEntity ;
  rdfs:label "Government Entity"@en ;
  rdfs:comment "A type of OrganizationalEntity related to the governance of an area."@en ;
  :wordnet_noun_synset "08180172", "08183086", "08183217", "08373001" .

:GroupOfAgents a owl:Class ;
  rdfs:subClassOf :Agent, :Collection ;
  rdfs:label "Group/Collection of Agents"@en ;
  rdfs:comment "A sub-class of both Agent and Collection defining a set/grouping of Agents."@en ;
  :example "Examples of a groups of Agents are OrganizationalEntity, or the concept of a family. However, even an indistinct 'mob' is classified as a group of Agents, as well as the 'population' of a region."@en ;
  :wordnet_noun_synset "07967506", "07991473" .

:JudicialGroup a owl:Class ;
  rdfs:subClassOf :GovernmentalEntity ;
  rdfs:label "Judicial Group"@en ;
  rdfs:comment "A type of GovernmentalEntity responsible for interpreting laws, and applying them to individual cases."@en .

:LineOfBusiness a owl:Class ;
  rdfs:label "Line/Type of Business"@en ;
  rdfs:comment "Indicates different types of industries/lines of business that may be the focus of an Agent (typically a Person or OrganizationalEntity). Note that LineOfBusiness is intended to be an abstract superclass (i.e., it should not be instantiated). Its subclasses (such as Agribusiness or TransportBusiness) define the specific semantics. These subclasses are directly referenced when used in a :has_line_of_business triple, via OWL punning."@en ;
  :wordnet_noun_synset "01099024", "01096649", "00583425", "00584498", "00611221", "08082070" .

:OrganizationalEntity a owl:Class ;
  rdfs:subClassOf :GroupOfAgents ;
  rdfs:label "Organizational Entity"@en ;
  rdfs:comment "As defined by Wikipedia (https://en.wikipedia.org/w/index.php?title=Organization&oldid=932509999), an organization 'is an entity comprising multiple people, such as an institution or an association, that has a particular purpose'. Note that OrganizationalEntities can themselves contain OrganizationalEntities, which are typically referred to as 'organizational units', or GroupsOfAgents such as project teams."@en .

:ParamilitaryAndRebelForce a owl:Class ;
  rdfs:subClassOf :OrganizationalEntity ;
  rdfs:label "Paramilitary and Rebel Force"@en ;
  rdfs:comment "From Wikipedia (https://en.wikipedia.org/w/index.php?title=Paramilitary&oldid=1015705600), a paramilitary 'organization (also listed as quasi military) is a semi-militarized force whose organizational structure, tactics, training, subculture, and (often) function are similar to those of a professional military, but is not formally part of a country's armed forces'. This class also includes rebel 'armies'."@en ;
  :wordnet_noun_synset "08224130" .

:Person a owl:Class ;
  rdfs:subClassOf :Agent ;
  rdfs:label "Person"@en ;
  rdfs:comment "A human being."@en ;
  :wordnet_noun_synset "00007846" .

:PoliceForce a owl:Class ;
  rdfs:subClassOf :GovernmentalEntity ;
  rdfs:label "Police Force"@en ;
  rdfs:comment "From Wikipedia (https://en.wikipedia.org/w/index.php?title=Police&oldid=1018027470), Police 'are a constituted body of persons empowered by a state, with the aim to enforce the law, to ensure the safety, health and possessions of citizens, and to prevent crime and civil disorder. Their lawful powers include arrest and the use of force legitimized by the state via the monopoly on violence. The term is most commonly associated with the police forces of a sovereign state that are authorized to exercise the police power of that state within a defined legal or territorial area of responsibility.'"@en ;
  :wordnet_noun_synset "08226608", "08228211" .

:PoliticalGroup a owl:Class ;
  rdfs:subClassOf :GroupOfAgents ;
  rdfs:label "Political Ideology"@en ;
  rdfs:comment "A PoliticalGroup is a set of persons with a common political ideology. From Wikipedia (https://en.wikipedia.org/w/index.php?title=List_of_political_ideologies&oldid=1017695528), a political ideology is a 'certain set of ethical ideals, principles, doctrines, myths or symbols of a social movement, institution, class or large group that explains how society should work and offers some political and cultural blueprint for a certain social order. A political ideology largely concerns itself with how to allocate power and to what ends it should be used. Some political parties follow a certain ideology very closely while others may take broad inspiration from a group of related ideologies without specifically embracing any one of them ... Political ideologies have two dimensions: (1) goals: how society should be organized; and (2) methods: the most appropriate way to achieve [these goals].' A Location or Agent may be associated with an ideology using the :has_political_ideology property."@en ;
  :example "Examples are groups of persons who identify as Democrats or Republicans."@en ;
  :wordnet_noun_synset "06222574" .

:PoliticalParty a owl:Class ;
  rdfs:subClassOf :OrganizationalEntity ;
  rdfs:label "Political Party"@en ;
  rdfs:comment "An organized group of Persons with similar opinions and goals related to how governement and society should be structured and operate. PoliticalParties work to get their candidates elected to political office."@en ;
  :wordnet_noun_synset "08273889" .

:ReligiousGroup a owl:Class ;
  rdfs:subClassOf :GroupOfAgents ;
  rdfs:label "Religious Group"@en ;
  rdfs:comment "A set of persons with common religious beliefs."@en .

:SocialGroup a owl:Class ;
  rdfs:subClassOf :OrganizationalEntity ;
  rdfs:label "Social Group"@en ;
  rdfs:comment "An organized group for social activities such as a bridge club, bowling league, etc."@en .


########################################################################
# Datatype Properties
########################################################################
  
:gender a owl:DatatypeProperty, owl:FunctionalProperty ;
  rdfs:label "gender"@en ;
  rdfs:domain :Person ;
  rdfs:range [ a rdfs:Datatype ;
               owl:onDatatype xsd:string ;
               owl:oneOf  ('binary' 'female' 'male' 'non-binary') ] ;
  rdfs:comment "String restricted to a set of values that indicating a Person's identified gender. The possible values are 'binary' 'female' 'male' 'non-binary'."@en .

:line_of_business a owl:DatatypeProperty ;
  rdfs:label "line of business"@en ;
  rdfs:domain :Agent ;
  rdfs:range xsd:string ;
  rdfs:comment "Specifies a particular type/line of business (as free form text) that is the focus of an Agent (typically a Person or OrganizationalEntity). Note that the :has_line_of_business property may also be specified, which maps the text to a set of predefined values."@en .

:role a owl:DatatypeProperty ;
  rdfs:label "role"@en ;
  rdfs:range xsd:string ;
  rdfs:comment "Specifies a function (as free-form text) that an Agent 'plays' in an Affiliation, to which an Agent is appointed/nominated or with a specific set of duties, privileges and responsibilities. It is specified as an edge property on an :affiliated relationship."@en .

:years_education a owl:DatatypeProperty, owl:FunctionalProperty ;
  rdfs:label "years of education"@en ;
  rdfs:domain :Person ;
  rdfs:range [ a rdfs:Datatype ;
               owl:onDatatype xsd:integer ;
               owl:withRestrictions ( [ xsd:minInclusive "0"^^xsd:integer ] ) ] ;
  rdfs:comment "Non-negative integer indicating the (estimated) years of schooling of a Person."@en .


########################################################################
# Object Properties
########################################################################

:affiliated a owl:ObjectProperty ;
  rdfs:label "has citizenship"@en ;
  rdfs:domain :Person ;
  rdfs:comment "Relationship indicating that the referencing Person is associated with another entity, such as another Agent, OrganizationalEntity or Location. The time of the Affiliation can be specified using the :has_time property (or one of its subproperties) as an RDF* graph property on :affiliated. Another possibility is to use the :role property as another RDF* graph property. This permits the capture of the role of the Person, for the indicated time."@en ;
  :example "Examples of Affiliations are a Person associated as an alumnus of their university, as an employee of a company, or as a member of a religious or political group."@en ;
  :wordnet_noun_synset "01083552" .

:has_citizenship a owl:ObjectProperty ;
  rdfs:label "has citizenship"@en ;
  rdfs:domain :Person ;
  rdfs:range :Country ;
  rdfs:comment "Indicates that the Person holds/held citizenship in the referenced Country. Note that a Person's citizenship may evolve over time as a Person changes residence, marries, etc. The time when a Person holds a particular citizenship may be defined using an RDF* graph property. In this case, the :has_time property or one of its sub-properties can be used with the :has_citizenship property."@en .

:has_line_of_business a owl:ObjectProperty ;
  rdfs:label "has line of business"@en ;
  rdfs:domain :Agent ;
  rdfs:range :LineOfBusiness ;
  rdfs:comment "References a particular type/line of business that is the focus of an Agent (typically a Person or OrganizationalEntity). Note that the :line_of_business property may also be specified, indicating an unmapped value or the type of business using the specific vocabulary/text of the narrative"@en .


########################################################################
# Subclasses of LineOfBusiness
########################################################################

:Agribusiness a owl:Class ;
  rdfs:subClassOf :LineOfBusiness ;
  rdfs:label "Agribusiness"@en ;
  rdfs:comment "Involved with the production of food by raising crops, plants, seeds, fish, insects and/or animals."@en ;
  :wordnet_noun_synset "01106311", "00454755", "00918116", "00917978", "00918295", "00916760", "00917553", "00919445", "00920103", "08092123", "01129030" .

:ArtsLiteratureAndMusic a owl:Class ;
  rdfs:subClassOf :EntertainmentBusiness ;
  rdfs:label "Arts, Literature and Music"@en ;
  rdfs:comment "Creativity expressed as painting, sculpture, writing, etc."@en .

:BankingAndFinanceBusiness a owl:Class ;
  rdfs:subClassOf :LineOfBusiness ;
  rdfs:label "Banking, Finance and Investment Business"@en ;
  rdfs:comment "Involved with the management of cash, credit and financial transactions by commerical and central banks, wealth management firms, stock traders and stock trading activities, bankers, tellers, etc."@en ;
  :wordnet_noun_synset "01100603", "01102563", "08083327", "08086714", "08087686" .

:ConstructionBusiness a owl:Class ;
  rdfs:subClassOf :ManufacturingBusiness ;
  rdfs:label "Construction Business"@en ;
  rdfs:comment "Involved in the building, maintenance and repair of infrasturcture, public and private spaces, and residential and commerical structures/buildings."@en ;
  :wordnet_noun_synset "01106542", "08084519" .

:CriminalBusiness a owl:Class ;
  rdfs:subClassOf :LineOfBusiness ;
  rdfs:label "Criminal Business"@en ;
  :wordnet_noun_synset "01114037", "08261980", "08262093", "08262346", "08263223", "08260983", "08262723" .

:EducationalBusiness a owl:Class ;
  rdfs:subClassOf :LineOfBusiness ;
  rdfs:label "Educational Business"@en ;
  rdfs:comment "Involved with the training/instruction of students regarding basic or advanced skills (from reading and writing to trades) and general or specific knowledge."@en ;
  :wordnet_noun_synset "00612720" .

:ElectronicsAndComputersBusiness a owl:Class ;
  rdfs:subClassOf :ScienceAndTechnologyBusiness ;
  rdfs:label "Electronics and Computers Related Business"@en ;
  rdfs:comment "Involved with the design and fabrication of transistors, microchips, semiconductors, etc and the devices made from those components."@en ;
  :example "Examples include both the engineering, fabrication and testing aspects of electronics and computer hardware."@en ;
  :wordnet_noun_synset "08084637", "08084401", "08019477", "08083801", "00952816" .

:EnergyAndUtilitiesBusiness a owl:Class ;
  rdfs:subClassOf :LineOfBusiness ;
  rdfs:label "Energy and Utilities Business"@en ;
  rdfs:comment "Involved with the infrastructure for and management of the supply of electricity, gas, water, waste, phone, cable, etc. to a community."@en ;
  :example "Examples are electrical, solar, wind and nuclear generator plants and businesses, water filtration actitivies, power distribution centers, garbage collection and recycling businesses, etc."@en ;
  :wordnet_noun_synset "00580371", "08084296", "08085886", "08086077", "08086323" .

:EntertainmentBusiness a owl:Class ;
  rdfs:subClassOf :LineOfBusiness ;
  rdfs:label "Entertainment Business"@en ;
  rdfs:comment "Involved with the creation, production, distribution and display/performance of film, music, art, sports, etc."@en ;
  :wordnet_noun_synset "08084787", "08084987", "03036237" .

:EnvironmentalOrEcologicalBusiness a owl:Class ;
  rdfs:subClassOf :LineOfBusiness ;
  rdfs:label "Environmental or Ecological Business"@en ;
  rdfs:comment "Involved with the preservation, protection and cleanup of the environment, flora and fauna, and with issues such as climate change."@en ;
  :wordnet_noun_synset "00277033", "14536664" .

:FashionBusiness a owl:Class ;
  rdfs:subClassOf :LineOfBusiness ;
  rdfs:label "Fashion Related Business"@en ;
  rdfs:comment "Involved with the design and production of clothing, footwear, accessories, beauty supplies, jewelry, etc."@en ;
  :wordnet_noun_synset "00609277", "08083153" .

:FoodProcessingAndPreparationBusiness a owl:Class ;
  rdfs:subClassOf :LineOfBusiness ;
  rdfs:label "Food Processing and Preparation Business"@en ;
  rdfs:comment "Involved with the 'transformation of agricultural products into food [or drink], or of one form of food into other forms. Food processing includes many forms ... from grinding grain to make raw flour to home cooking to complex industrial methods used to make convenience foods ... Primary food processing is necessary to make most foods edible, and secondary food processing turns the ingredients into familiar foods, such as bread.' (https://en.wikipedia.org/w/index.php?title=Food_processing&oldid=1013814848)"@en ;
  :example "Examples include bakeries, butcher shops and slaughterhouses, restaurants, etc."@en ;
  :wordnet_noun_synset "00621664", "01105869", "00717095", "08019869", "04088393" .

:GovernmentAndPoliticsBusiness a owl:Class ;
  rdfs:subClassOf :LineOfBusiness ;
  rdfs:label "Government and Politics Business"@en ;
  rdfs:comment "Involved with governing bodies and agencies, parliaments and law making, political parties, elected officials, etc."@en ;
  :wordnet_noun_synset "00613259" .

:HealthcareAndMedicalBusiness a owl:Class ;
  rdfs:subClassOf :LineOfBusiness ;
  rdfs:label "Healthcare and Medical Business"@en ;
  rdfs:comment "Involved with 'the maintenance or improvement of health via the prevention, diagnosis, treatment, recovery, or cure of disease, illness, injury, and other physical and mental impairments in people. Health care is delivered by health professionals and allied health fields.' (https://en.wikipedia.org/w/index.php?title=Health_care&oldid=1013329520)"@en ;
  :example "Medicine, dentistry, pharmacy, midwifery, nursing, optometry, audiology, psychology, occupational therapy, physical therapy, athletic training and other health professions are all part of health care. It includes work done in providing primary care, secondary care, and tertiary care, as well as in public health. (https://en.wikipedia.org/w/index.php?title=Health_care&oldid=1013329520)"@en ;
  :wordnet_noun_synset "00613447", "08019020", "08129596" .

:HospitalityBusiness a owl:Class ;
  rdfs:subClassOf :LineOfBusiness ;
  rdfs:label "Hospitality Business"@en ;
  rdfs:comment "Involved with food and drink services (performed by wait staff, attendants, etc.), lodging, amusement and theme parks, tour guides and services, travel agencies, etc."@en ;
  :wordnet_noun_synset "00298987", "01106229" .

:HumanitarianBusiness a owl:Class ;
  rdfs:subClassOf :LineOfBusiness ;
  rdfs:label "Humanitarian Business"@en ;
  rdfs:comment "Involved with providing direct services or materials to people and areas in need."@en ;
  :wordnet_noun_synset "01139918", "08026566" .

:InsuranceBusiness a owl:Class ;
  rdfs:subClassOf :LineOfBusiness ;
  rdfs:label "Insurance Business"@en ;
  rdfs:comment "Involved with protecting against financial loss related to damage to an asset or person."@en ;
  :wordnet_noun_synset "08087301" .

:LaborAndStaffingBusiness a owl:Class ;
  rdfs:subClassOf :LineOfBusiness ;
  rdfs:label "Labor and Staffing Business"@en ;
  rdfs:comment "Involved with organized labor, labor arbitration, providing or finding temporary or permanent staffing, etc."@en ;
  :wordnet_noun_synset "08371279" .

:LegalAndJudicialBusiness a owl:Class ;
  rdfs:subClassOf :LineOfBusiness ;
  rdfs:label "Legal and Judicial Business"@en ;
  rdfs:comment "Involved with courts/trials/litigations, etc."@en ;
  :wordnet_noun_synset "00612411", "08080875", "08129368", "08346380", "01189300" .

:ManufacturingBusiness a owl:Class ;
  rdfs:subClassOf :LineOfBusiness ;
  rdfs:label "Manufacturing Business"@en ;
  rdfs:comment "Involved with 'the production of goods through the use of labor, machines, tools, and chemical or biological processing or formulation ... The term may refer to a range of human activity, from handicraft to high-tech, but it is most commonly applied to industrial design, in which raw materials from the primary sector are transformed into finished goods on a large scale. Such goods may be sold to other manufacturers for the production of other more complex products (such as aircraft, household appliances, furniture, sports equipment or automobiles), or distributed via the tertiary industry to end users and consumers (usually through wholesalers, who in turn sell to retailers, who then sell them to individual customers). Manufacturing engineering, or the manufacturing process, are the steps through which raw materials are transformed into a final product. The manufacturing process begins with the product design, and materials specification from which the product is made. These materials are then modified through manufacturing processes to become the required part.' (https://en.wikipedia.org/w/index.php?title=Manufacturing&oldid=1013964157)"@en ;
  :wordnet_noun_synset "08077282", "08083913", "08085624", "08085760" .

:MilitaryAndSecurityBusiness a owl:Class ;
  rdfs:subClassOf :LineOfBusiness ;
  rdfs:label "Military and Security Related Business"@en ;
  rdfs:comment "Involved with the protection of (online and physical) locations, goods or persons via services and personnel and/or the armed forces, troops/officers/enlisted/non-coms, equipment and research/consulting related to these."@en ;
  :wordnet_noun_synset "01112538", "08227903" .

:MultiIndustryBusiness a owl:Class ;
  rdfs:subClassOf :LineOfBusiness ;
  rdfs:label "Multiple Industries Business"@en ;
  rdfs:comment "Involved with more than one line of business such as an industrial conglomerate."@en ;
  :wordnet_noun_synset "08075773" .

:ProvisionOfServicesBusiness a owl:Class ;
  rdfs:subClassOf :LineOfBusiness ;
  rdfs:label "Provision of Services Business"@en ;
  rdfs:comment "Involved with the sale of services to a business, person or group."@en ;
  :example "Examples are companies or individuals that provide education/training or IT/programming services."@en ;
  :wordnet_noun_synset "01105693", "00586211", "08086178", "08086463", "08090536" .

:PublishingAndMediaBusiness a owl:Class ;
  rdfs:subClassOf :LineOfBusiness ;
  rdfs:label "Publishing and Media Business"@en ;
  rdfs:comment "Involved with the creation, production, marketing and distribution of written and visual material."@en ;
  :example "Examples are activities related to creating and releasing books, journals, magazines, periodicals, blogs, newspapers, etc."@en ;
  :wordnet_noun_synset "00612961", "00613161", "00926528", "08018457", "08019615" .

:RawMaterialProcessingAndPreparationBusiness a owl:Class ;
  rdfs:subClassOf :LineOfBusiness ;
  rdfs:label "Raw Material Processing and Preparation Business"@en ;
  rdfs:comment "Involved with substances 'used to produce goods, finished products, energy, or intermediate materials that are feedstock for future finished products. As feedstock, the term connotes these materials are bottleneck assets and are required to produce other products. The term raw material denotes materials in unprocessed or minimally processed states; e.g., raw latex, crude oil, cotton, coal, raw biomass, iron ore, air, logs, water, or \"any product of agriculture, forestry, fishing or mineral in its natural form or which has undergone the transformation required to prepare it for international marketing in substantial volumes\".' (https://en.wikipedia.org/w/index.php?title=Raw_material&oldid=1014281791)"@en ;
  :example "Examples are mining, drilling/boring/reaming, logging, fishing and processing such as distillation and refinery."@en ;
  :wordnet_noun_synset "00455145", "08020061", "08020281" .

:RealEstateBusiness a owl:Class ;
  rdfs:subClassOf :LineOfBusiness ;
  rdfs:label "Real Estate Business"@en ;
  rdfs:comment "Involved with the maintenance and sale of property/land and buildings."@en ;
  :wordnet_noun_synset "01103132" .

:ReligiousBusiness a owl:Class ;
  rdfs:subClassOf :LineOfBusiness ;
  rdfs:label "Religious/Religion Related Business"@en ;
  rdfs:comment "Involved with activities related to spirituality, faith and worship."@en ;
  :example "Examples include churches and similar organizations."@en ;
  :wordnet_noun_synset "08130409", "03959692" .

:RetailBusiness a owl:Class ;
  rdfs:subClassOf :LineOfBusiness ;
  rdfs:label "Retail Business"@en ;
  rdfs:comment "Involved with the sale of goods on a small scale to end-users and direct consumers (versus for resale)."@en ;
  :example "Examples are stores, malls, groceries, etc."@en ;
  :wordnet_noun_synset "01103019", "04209460" .

:StorageBusiness a owl:Class ;
  rdfs:subClassOf :LineOfBusiness ;
  rdfs:label "Storage Business"@en ;
  rdfs:comment "A business related to the storing of goods, materials, foods, etc."@en ;
  :wordnet_noun_synset "00813322" .

:ScienceAndTechnologyBusiness a owl:Class ;
  rdfs:subClassOf :LineOfBusiness ;
  rdfs:label "Science and Technology Business"@en ;
  rdfs:comment "Involved with using knowledge (especially scientific knowledge) and incorporating it in machines. 'Systems (e.g. machines) applying technology by taking an input, changing it according to the system's use, and then producing an outcome are referred to as technology systems or technological systems.' (https://en.wikipedia.org/w/index.php?title=Technology&oldid=1051447059)"@en .

:TradeAndCraft a owl:Class ;
  rdfs:subClassOf :LineOfBusiness ;
  rdfs:label "Trade and Craft"@en ;
  rdfs:comment "Involved with making items or performing a job requiring skill and training."@en .

:TransportBusiness a owl:Class ;
  rdfs:subClassOf :LineOfBusiness ;
  rdfs:label "Transport Related Business"@en ;
  rdfs:comment "Involved with the logistics and movement of goods, humans, plants and/or animals to/from different locations, as performed by dock workers, truckers/long haulers/drivers, shippers, receivers, transporters, etc."@en ;
  :wordnet_noun_synset "01107164", "01113655", "01113857", "08020159", "08020531", "08020652", "08091976" .
