@prefix : <urn:ontoinsights:dna:> .
@prefix dna: <urn:ontoinsights:dna:> .
@prefix owl: <http://www.w3.org/2002/07/owl#> .
@prefix rdf: <http://www.w3.org/1999/02/22-rdf-syntax-ns#> .
@prefix rdfs: <http://www.w3.org/2000/01/rdf-schema#> .
@prefix xsd: <http://www.w3.org/2001/XMLSchema#> .

########################################################################
# File defining semantics related to different types of communications
# and speech acts (e.g., sub-classes of CommunicationAndSpeechAct).
# 
# These subclasses should be extended as needed for a domain of interest.
# 
# Created: April 1 2021
# Last Modified: December 11 2023
# 
# Licensed by OntoInsights, LLC
# Creative Commons Attribution 4.0 International (CC BY 4.0)
# 
# Unless required by applicable law or agreed to in writing,
# software distributed under the License is distributed on an
# "AS IS" BASIS, WITHOUT WARRANTIES OR CONDITIONS OF ANY KIND,
# either express or implied.
# 
# Changes:
#  Reset change history and simplified, Nov 2023
#  Corrected subclassing of :SurrenderAndYielding
#  Added :CourtRuling, :Debate, :Insult, :Polling
#  Clarified/corrected several descriptions
########################################################################


########################################################################
# Classes
########################################################################

:Acknowledgment a owl:Class ;
  rdfs:subClassOf :AssertionAndDeclaration ;
  rdfs:label "Acknowledgment"@en ;
  rdfs:comment "An admission of responsibility or guilt for some act. The Agent making the admission is indicated using the :has_active_entity property, while the thing that is confessed is defined using :has_topic."@en ;
  :wordnet_noun_synset "06641368", "07194603", "06483913", "07230608", "00154781", "07217786" ;
  :wordnet_verb_synset "00449245", "00818972" .

:AdviceAndRecommendation a owl:Class ;
  rdfs:subClassOf :CommunicationAndSpeechAct ;
  rdfs:label "Advice and Recommendation"@en ;
  rdfs:comment "An act of recommending or suggesting something. The Agent doing the communicating is indicated using the :has_active_entity property, while the entity being advised is defined using :has_affected_entity."@en ;
  :wordnet_noun_synset "06684229", "05924749", "09793689", "06663446" ;
  :wordnet_verb_synset "02444597", "02003830", "00876925", "00876672", "00877973", "00878196" .

:AppointmentAndNomination a owl:Class ;
  rdfs:subClassOf :AssertionAndDeclaration ;
  rdfs:label "Appointment and Nomination"@en ;
  rdfs:comment "An act of proposing an Agent for a task or position. The Agent doing the proposing is indicated using the :has_active_entity property, while the Agent being appointed/nominated is defined using :has_affected_entity."@en ;
  :wordnet_noun_synset "00164600", "01142792" ;
  :wordnet_verb_synset "02401347", "00881061", "02480684" .

:AssertionAndDeclaration a owl:Class ;
  rdfs:subClassOf :CommunicationAndSpeechAct ;
  rdfs:label "Assertion and Declaration"@en ;
  rdfs:comment "A claim or statement of fact or of belief. The Agent making the declaration is indicated using the :has_active_entity property, while the entity discussed is defined using :has_topic."@en ;
  :wordnet_noun_synset "06699481", "06735202", "07216025", "07189892", "07214225", "07222998", "07226850", "07228055", "07245162", "07247081" ;
  :wordnet_verb_synset "00758383", "01018787", "01011267", "00833312", "00758383" .

:Challenge a owl:Class ;
  rdfs:subClassOf :RequestAndAppeal ;
  rdfs:label "Challenge"@en ;
  rdfs:comment "A request/invitation to take part in a contest or competition. The Agent issuing the challenge is indicated using the :has_active_entity property, while the Person who is challenged is defined using :has_affected_entity."@en ;
  :wordnet_noun_synset "07245954", "00790898" ;
  :wordnet_verb_synset "00870255", "01124374" .

:CitationAndReference a owl:Class ;
  rdfs:subClassOf :Acknowledgment ;
  rdfs:label "Citation and Reference"@en ;
  rdfs:comment "The act of referencing or quoting from a book, article, paper, ... and acknowledging that source."@en ;
  :wordnet_noun_synset "07195230", "07273332", "01032674" ;
  :wordnet_verb_synset "01025268", "01025583", "01709116".

:CommandAndDemand a owl:Class ;
  rdfs:subClassOf :RequestAndAppeal ;
  rdfs:label "Command and Demand"@en ;
  rdfs:comment "A communication that issues orders, mandates, etc. The Agent issuing the command/making the demand is indicated using the :has_active_entity property, while the Person with whom the Agent is communicating is defined using :has_affected_entity. The subject of the demand is specified using the :has_topic property."@en ;
  :wordnet_noun_synset "07182782", "00805278", "01217047", "07205939" ; 
  :wordnet_verb_synset "00749139", "02396945", "00748704", "00756987", "00718950" .

:Complaint a owl:Class ;
  rdfs:subClassOf :CommunicationAndSpeechAct ;
  rdfs:label "Complaint"@en ;
  rdfs:comment "An expression of displeasure or annoyance about something. The Agent doing the complaining is indicated using the :has_active_entity property, while the thing complained about is defined using :has_topic."@en ;
  :wordnet_noun_synset "07223368", "05741963", "07224625" ;
  :wordnet_verb_synset "00845977", "00909100", "00828170" .

:CourtOrderAndRuling a owl:Class ;
  rdfs:subClassOf :CommunicationAndSpeechAct, :LawRelated ;
  rdfs:label "Court Order and Ruling"@en ;
  rdfs:comment "A court's decision on a legal case or party's motion in a legal case, and/or an order for an entity to do or not do something. The court is indicated using the :has_active_entity property, while the legal case is defined using :has_topic. The decision is identified using :has_goal."@en .

:Debate a owl:Class ;
  rdfs:subClassOf :MeetingAndEncounter, :CommunicationAndSpeechAct ;
  rdfs:label "Debate"@en ;
  rdfs:comment "A discussion or competition considering one or more topics, where different individuals or teams present their positions. The persons/teams involved in a debate are indicated using the :has_active_entity property."@en .

:Denial a owl:Class ;
  rdfs:subClassOf :AssertionAndDeclaration ;
  rdfs:label "Denial"@en ;
  rdfs:comment "A claim that something is untrue. The Agent making the declaration is indicated using the :has_active_entity property, while the entity discussed is defined using :has_topic."@en ;
  :wordnet_noun_synset "07219061", "07247648" ;
  :wordnet_verb_synset "00818664", "00818217" . 

:ExpressiveAndExclamation a owl:Class ;
  rdfs:subClassOf :CommunicationAndSpeechAct ;
  rdfs:label "Expressive and Exclamation"@en ;
  rdfs:comment "Any statements that express attitude or emotion. The Agent making the declaration is indicated using the :has_active_entity property. The instance is also defined as a sub-class of EmotionalResponse to indicate the emotion that is expressed. Note that this kind of statement/sentence may include an exclamation point (!)."@en ;
  :wordnet_noun_synset "06642524", "06646403", "06646199", "06645870", "06646103", "06705943" ;
  :wordnet_verb_synset "00914001", "00894444", "00898638", "00898754" .

:Inquiry a owl:Class ;
  rdfs:subClassOf :CommunicationAndSpeechAct ;
  rdfs:label "Inquiry"@en ;
  rdfs:comment "A CommunicationAndSpeechAct involving asking questions/for information. The Agent making the inquiry is indicated using the :has_active_entity property. The thing that is inquired about is indicated using :has_topic."@en ;
  :wordnet_noun_synset "07207844", "07208618" ; 
  :wordnet_verb_synset "00899241", "00788478" .

:Insult a owl:Class ;
  rdfs:subClassOf :CommunicationAndSpeechAct ;
  rdfs:label "Insult"@en ;
  rdfs:comment "An act of being verbally disrespectful, scornful or abusive. The Agent doing the insulting is indicated using the :has_active_entity property, while the Agent being insulted is defined using :has_affected_entity."@en .

:Permission a owl:Class ;
  rdfs:subClassOf :CommunicationAndSpeechAct ;
  rdfs:label "Permission"@en ;
  rdfs:comment "An act of allowing or authorizing something to occur. The thing that is allowed is indicated using the :has_topic property."@en ;
  :wordnet_noun_synset "01141515" ;
  :wordnet_verb_synset "02479404", "00803980", "02449527" .

:Polling a owl:Class ;
  rdfs:subClassOf :Inquiry ;
  rdfs:label "Polling"@en ;
  rdfs:comment "An act of inquiry in order to obtain the opinion and thoughts of a set of people."@en .

:PromiseAndOath a owl:Class ;
  rdfs:subClassOf :AssertionAndDeclaration, :Agreement ;
  rdfs:label "Promise and Oath"@en ;
  rdfs:comment "An act of allowing or authorizing something to occur. The thing that is allowed is indicated using the :has_topic property."@en ;
  :wordnet_noun_synset "07241205", "07242432", "01208643", "01242433" ;
  :wordnet_verb_synset "00888280", "00885532", "00885838", "00886738" .

:RefusalAndRejection a owl:Class ;
  rdfs:subClassOf :CommunicationAndSpeechAct ;
  rdfs:label "Refusal and Rejection"@en ;
  rdfs:comment "An act related to not accepting or acknowledging something, someone, or some Event or StateAndCondition. The entity that is not acknowledged/accepted is identified using the :has_topic predicate."@en ;
   :wordnet_noun_synset "07221933", "06646602", "01228486", "01228670", "00204191", "07270069", "00202772", "01228272" ; 
   :wordnet_verb_synset "00799092", "00687584", "00797525", "00808840", "00798638" .

:RequestAndAppeal a owl:Class ;
  rdfs:subClassOf :CommunicationAndSpeechAct ;
  rdfs:label "Request and Appeal"@en ;
  rdfs:comment "A CommunicationAndSpeechAct that expresses a need or desire for something or someone, or that some event or condition occur. Note that who/what is requested is identified using the :has_topic predicate."@en ;
  :wordnet_noun_synset "07199985", "06525357", "01044000", "07201488" ;
  :wordnet_verb_synset "00747485", "00754499", "00754770", "00761314", "00757492", "00895886", "02275660" .

:SurrenderAndYielding a owl:Class ;
  rdfs:subClassOf :AssertionAndDeclaration, :Loss ;
  rdfs:label "Surrender and Yielding"@en ;
  rdfs:comment "An act where one Agent admits/concedes defeat and/or agrees to give up fighting or to relinquish power, possession or control of something to another."@en ;
  :wordnet_noun_synset "00068527", "06523753", "07269504", "00213657", "07269262" ;
  :wordnet_verb_synset "01118865", "00806138", "02384340", "02232523", "02240011", "02709149", "00805801" .

:ThreatAndWarning a owl:Class ;
  rdfs:subClassOf :CommunicationAndSpeechAct, :CoercionAndIntimidation ;
  rdfs:label "Threat and Warning"@en ;
  rdfs:comment "A CommunicationAndSpeechAct intended to frighten by expressing the intention to take action in response to something (some Event) done or not done. The Event that is done/not done is specified using the :has_topic predicate. The Agent who is making the threats is defined using :has_active_entity, while the threatened Agent is identified using :has_affected_entity."@en ;
  :wordnet_noun_synset "06746225", "00786042" ; 
  :wordnet_verb_synset "00871877", "00012130", "01069216", "01784999", "02246403" .


########################################################################
# Disjointness
########################################################################

[] rdf:type owl:AllDisjointClasses ;
  owl:members  ( :Acknowledgment :Denial ) .

[] rdf:type owl:AllDisjointClasses ;
  owl:members  ( :Permission :RefusalAndRejection ) .
