@prefix : <urn:ontoinsights:dna:> .
@prefix dna: <urn:ontoinsights:dna:> .
@prefix owl: <http://www.w3.org/2002/07/owl#> .
@prefix rdf: <http://www.w3.org/1999/02/22-rdf-syntax-ns#> .
@prefix rdfs: <http://www.w3.org/2000/01/rdf-schema#> .
@prefix xsd: <http://www.w3.org/2001/XMLSchema#> .

########################################################################
# File defining semantics related to specific events/actions/occurrences.
# 
# The subclasses of Event should be extended as needed for a domain
# of interest.
# 
# Created: April 1 2021
# Last Modified: March 1 2024
# 
# Licensed by OntoInsights, LLC
# Creative Commons Attribution 4.0 International (CC BY 4.0)
# 
# Unless required by applicable law or agreed to in writing,
# software distributed under the License is distributed on an
# "AS IS" BASIS, WITHOUT WARRANTIES OR CONDITIONS OF ANY KIND,
# either express or implied.
# 
# Changes:
#  Reset change history and simplified
#  Modified superclasses for several classes
#  Acquisition renamed to AcquisitionPossessionAndTransfer; Possession
#    and ChangeOfPossession merged into this semantic
#  Removed ViolationOfAgreement and merged its semantics with
#    DisagreementAndDispute
#  Added Commemoration and EducationEvent
#  Removed Rally and merged its semantic into DemonstrationStrikeAndRally
#  Clarified FinancialEvent to become EconomyAndFinanceRelated
#  Moved InformationHandling into the semantics of a new class, 
#    TechnologyRelated
#  Removed ProjectAndCampaign since its semantics are addressed by
#     GoalDirectedProcess (defined in top.ttl)
#  Removed RecreationAndSportEvent and merged its semantic into
#    ArtAndEntertainmentEvent
#  Expanded ReligiousCeremony to a more general ReligiousEvent
#  Moved (from misc-event-subclasses.ttl), clarified and renamed 
#    CaptureAndSeizure and CaptivityAndDetention (from environment-
#    subclasses.ttl) to become ArrestAndImprisonment
########################################################################


########################################################################
# Classes
########################################################################

:AcquisitionPossessionAndTransfer a owl:Class ;
  rdfs:subClassOf :EventAndState ;
  rdfs:label "Acquisition, Possession and Transfer"@en ;
  rdfs:comment "The acquiring/obtaining and possessing of some object/asset/knowledge/skill. Subclasses indicate whether this occurred by a gift, purchase, recovered item, theft, etc. In addition, acquisition implies having or controlling some object or asset (e.g., possession). However, possession may or may not indicate ownership."@en ;
  :wordnet_noun_synset "14503072", "00032912", "00811126", "00812259", "13261412", "00042637", "00043933", "14502904", "09783624" ;
  :wordnet_verb_synset "02209474", "02306641", "02215637", "00723361", "01216829", "02320505", "02352633" .

:AggressiveCriminalOrHostileAct a owl:Class ;
  rdfs:subClassOf :EventAndState ;
  rdfs:label "Aggressive, Criminal or Hostile Act"@en ;
  rdfs:comment "Unfriendly, offensive, damaging, belligerent and/or criminal actions or statements. Note that if the Event involved a statement/communication, then the individual should also be classified as a :CommunicationAndSpeechAct."@en ;
  :wordnet_noun_synset "14004330", "00966680", "01224100", "07563271", "00734044" ;
  :wordnet_verb_synset "01793315", "01811281", "01827478", "02519655" .

:Agreement a owl:Class ;
  rdfs:subClassOf :EventAndState ;
  rdfs:label "Agreement"@en ;
  rdfs:comment "Events where two or more Agents share the same opinion and/or make arrangements (perhaps legally) to do something. Note that the property, :has_topic, indicates 'what is agreed to' and the involved Agents are identified using the :has_active_agent predicate."@en ;
  :wordnet_noun_synset "06783066", "13992690", "01217882" ;
  :wordnet_verb_synset "00799359", "00766267", "00559750" .

:AgricultureApicultureAndAquacultureEvent a owl:Class ;
  rdfs:subClassOf :EventAndState ;
  rdfs:label "Agriculture, Apiculture, Aquaculture and Viticulture Event"@en ;
  rdfs:comment "Events dealing with farming, ranching, breeding, beekeeping, etc."@en ;
  :wordnet_verb_synset "01746607", "01383909", "02425530", "00056076", "01322669" .

:Alignment a owl:Class ;
  rdfs:subClassOf :InclusionAttachmentAndUnification ;
  rdfs:label "Alignment"@en ;
  rdfs:comment "A type of grouping related to the arranging or organizing of the component entities."@en ;
  :wordnet_noun_synset "05082771" ;
  :wordnet_verb_synset "01466592" .

:ArrestAndImprisonment a owl:Class ;
  rdfs:subClassOf :RemovalAndRestriction ;
  rdfs:label "Arrest and Incarceration"@en ;
  rdfs:comment "An act involving the taking and/or detention of a Person by authority of the law. However, imprisonment may also not be authorized and reflect an illegal act. In the case of the latter, the event should also be an instance of AggressiveCriminalorHostileAct. The Agent who performs the arrest or imprisonment is specified using the :has_active_agent property, while the Person(s) who are arrested/imprisoned are identified using :has_affected_agent."@en ;
  :wordnet_noun_synset "00089545", "01149281", "14020535", "01149089" ;
  :wordnet_verb_synset "01217701", "02500005", "02500687", "02502345" .

:ArtAndEntertainmentEvent a owl:Class ;
  rdfs:subClassOf :EventAndState ;
  rdfs:label "Art and Entertainment Event"@en ;
  rdfs:comment "Events involved with the display and/or performance of art, music, films, plays, etc., as well as other occurrences such as sporting events. These activities are 'observed' by Agents for enjoyment (who are indicated using the :has_affected_agent predicate) and may be 'performed by' other Agents (specified using the :has_active_agent property)."@en ;
  :wordnet_noun_synset "00427931", "00402591", "00041926", "00456623" ;
  :wordnet_verb_synset "00013321", "01075360", "01151936", "02423521", "01718067", "02497847", "01727101" .

:AssessmentMeasurement a owl:Class ;
  rdfs:subClassOf :Measurement ;
  rdfs:label "Assessment Measurement"@en ;
  rdfs:comment "A type of Measurement describing an event or situation (such as Employment in a Country) with a restricted set of reported values. The assessment scale varies from 'negligible or none' to 'very high'. The reported value is specified using the :assessment property."@en .

:Attempt a owl:Class ;
  rdfs:subClassOf :EventAndState ;
  rdfs:label "Attempt"@en ;
  rdfs:comment "Attempt should not be used alone to classify an individual. Another Event subclass should also be specified. Attempt indicates that an effort was made to do/complete the 'other' Event, but it did not succeed/was not accomplished."@en ;
  :wordnet_noun_synset "00787849" ; 
  :wordnet_verb_synset "01654835", "02535833", "01148517" .

:Avoidance a owl:Class ;
  rdfs:subClassOf :EventAndState ;
  rdfs:label "Avoidance"@en ;
  rdfs:comment "The act of staying away from some object or Agent, purposefully not doing something or preventing something from occurring."@en ;
  :wordnet_noun_synset "00204602", "01070697", "04889817", "01068613" ;
  :wordnet_verb_synset "00813037", "01198570", "02731589" .

:Birth a owl:Class ;
  rdfs:subClassOf :LifeEvent, :StartAndBeginning ;
  rdfs:label "Birth"@en ;
  rdfs:comment "An individual (living entity) being born/beginning life."@en ;
  :wordnet_noun_synset "07334902" ;
  :wordnet_verb_synset "00056644" .

:BodilyAct a owl:Class ;
  rdfs:subClassOf :EventAndState ;
  rdfs:label "Bodily Act"@en ;
  rdfs:comment "An activity typically involving the body of an animal or Person (such as coughing, eating or running)."@en ;
  :wordnet_noun_synset "13461236" ;
  :wordnet_verb_synset "00072742" .

:Bribe a owl:Class ;
  rdfs:subClassOf :RewardAndCompensation ;
  rdfs:label "Bribe"@en ;
  rdfs:comment "Offering of money or thing(s) of value to induce a Person to perform certain actions."@en ;
  :wordnet_noun_synset "00777759" ;
  :wordnet_verb_synset "02288941" . 

:Ceremony a owl:Class ;
  rdfs:subClassOf :MeetingAndEncounter ;
  rdfs:label "Ceremony"@en ;
  rdfs:comment "A gathering to formally/officially highlight an occurrence of importance (such as a wedding, funeral or the opening of a facility) or to remember a previous event (such as a birthday or historical Event). The occurrence being highlighted or remembered is identified using the :has_topic predicate."@en ;
  :wordnet_noun_synset "01029321", "01028839", "7465442" ; 
  :wordnet_verb_synset "00614139", "02400924", "02430184" .

:Change a owl:Class ;
  rdfs:subClassOf :EventAndState ;
  rdfs:label "Change"@en ;
  rdfs:comment "Indicates a difference in the availability/count/amount of something or in the demeanor/behavior of an Agent. The thing/Agent which 'changes' is referenced using the :has_topic property. Note that two subclasses are defined, Increase and Decrease. The pace of the Change can be described using an associated instance of :AssessmentMeasurement (associated using the :has_measurement property)."@en ;
  :example "Examples are changes in the amount of something (such as food, water or schools), an increase/decrease in the number of certain types of Events (such as murders) or available teachers (a GroupOfAgents with the :has_line_of_business predicate set to :EducationalBusiness and the :prototypical property set to true), etc."@en ;
  :wordnet_noun_synset "00169459", "14057399", "06207399", "00191991" ;
  :wordnet_verb_synset "00109468" .

:Cognition a owl:Class ;
  rdfs:subClassOf :EventAndState ;
  rdfs:label "Cognition"@en ;
  rdfs:comment "Any thought processes related to learning, making decisions, perception, memory, imagination, forming judgments, etc. Note that the Person who is thinking is defined using the :has_active_agent property. And, details about what is learned/thought/understood is indicated using the :has_topic predicate."@en ;
  :wordnet_noun_synset "05682974", "00023451", "05658174", "05778923", "04667893", "05716379" ;
  :wordnet_verb_synset "00691086", "00630153" .

:Commemoration a owl:Class ;
  rdfs:subClassOf :EventAndState ;
  rdfs:label "Commemoration"@en ;
  rdfs:comment "An event that remembers and respects someone, something or some occurrence in the past. The thing that is remembered is identified using the :has_topic property. The Person who is remembering is indicated using the :has_active_agent property."@en ;
  :wordnet_noun_synset "06701267" ;
  :wordnet_verb_synset "00613035" . 

:CommunicationAndSpeechAct a owl:Class ;
  rdfs:subClassOf :EventAndState ;
  rdfs:label "Communication and Speech Act"@en ;
  rdfs:comment "Any act of conveying information via written or spoken word, or non-verbal means. The Agent doing the communicating is indicated using the :has_active_agent property, while the entity listening is defined using :has_affected_agent."@en ;
  :wordnet_noun_synset "07253354" ;
  :wordnet_verb_synset "00800905", "00817348", "00742582", "0074428" . 

:Competition a owl:Class ;
  rdfs:subClassOf :EventAndState ;
  rdfs:label "Competition"@en ;
  rdfs:comment "An Event or ongoing condition where two or more Agents are striving for a similar goal (such as winning a contest or using scarce Resources), and want to be better/more successful than the others. This class refers to both specific competitive Events, as well as the general condition. The former would be Evidence for the latter. If competing over Resources, these are defined using the :has_topic predicate. The Agents are identified using the :has_agent property. The overall competitive situation can be described using an associated instance of :AssessmentMeasurement (associated using the :has_measurement property)."@en ;
  :wordnet_noun_synset "01171059", "07470961" ;
  :wordnet_verb_synset "01074673", "01081873" .

:Cooperation a owl:Class ;
  rdfs:subClassOf :FriendlyOrSupportiveAct ;
  rdfs:label "Cooperation"@en ;
  rdfs:comment "An Event or ongoing condition where two or more Agents are striving for a similar goal, and are mutually assisting/supporting one another. This class refers to both specific coooperative Events, as well as the general condition. The former would be Evidence for the latter. If cooperating/sharing Resources, these are defined using the :has_topic predicate. The Agents are identified using the :has_agent property.  The overall cooperative situation can be described using an associated instance of :AssessmentMeasurement (associated using the :has_measurement property)."@en ;
  :wordnet_noun_synset "00412397", "01205394", "13864062" ; 
  :wordnet_verb_synset "02421408", "02300511" .

:Coup a owl:Class ;
  rdfs:subClassOf :TransferOfPower ;
  rdfs:label "Coup"@en ;
  rdfs:comment "A seizure of power from an existing government, establishing a new one. The government which is overthrown is identified using the :has_affected_agent property, while the new regime is identified using :has_active_agent."@en ;
  :wordnet_noun_synset "01147528" ; 
  :wordnet_verb_synset "02407551", "02407837" .

:Death a owl:Class ;
  rdfs:subClassOf :LifeEvent, :End ;
  rdfs:label "Death"@en ;
  rdfs:comment "The end of a living entity's life."@en ;
  :wordnet_noun_synset "07370091", "07354694", "09919123", "15168437", "13985834" ;
  :wordnet_verb_synset "00359085" . 

:Decrease a owl:Class ;
  rdfs:subClassOf :Change ;
  rdfs:label "Decrease"@en ;
  rdfs:comment "Indicates a lowering/decline in the availability/count/amount of something or in the demeanor/behavior of an Agent. The pace of the Decrease can be described using an associated instance of :AssessmentMeasurement (associated using the :has_measurement property)."@en ;
  :wordnet_noun_synset "13496741", "00352464", "05117108", "13479774" ;
  :wordnet_verb_synset "00223926", "00045548", "00204228", "00269051", "00494865", "00432779", "00275432", "00275523" .

:DelayAndWait a owl:Class ;
  rdfs:subClassOf :EventAndState ;
  rdfs:label "Delay and Wait"@en ;
  rdfs:comment "A lack of action."@en ;
  :wordnet_noun_synset "01068087", "01065863" ;
  :wordnet_verb_synset "00460731", "02644022", "02648898" . 

:DemonstrationStrikeAndRally a owl:Class ;
  rdfs:subClassOf :MeetingAndEncounter ;
  rdfs:label "Demonstration, Strike and Rally"@en ;
  rdfs:comment "A meeting to support or object to something, someone or some cause. The thing or Agent which is the focus of the Event is defined using the :has_topic property.  Note that these types of events can be supportive or show opposition. It is recommended that an Event classified as a rally should also be typed as either a :FriendlyOrSupportiveAct or a :DisagreementOrDispute."@en ;
  :wordnet_noun_synset "08375259", "01180193", "01170859", "01180685", "01245509", "01244711", "01181340" ;
  :wordnet_verb_synset "02417777", "02527482"  .

:DisagreementAndDispute a owl:Class ;
  rdfs:subClassOf :EventAndState ;
  rdfs:label "Disagreement and Dispute"@en ;
  rdfs:comment "Events where two or more Agents do NOT share the same opinion and argue. Note that the property, :has_topic, indicates 'what is in disagreement' and the involved Agents are identified using the :has_active_agent predicate. This semantic may also be used to indicate that an agreement has been violated/is 'in dispute' where the agreement is indicated using :has_topic."@en ;
  :wordnet_noun_synset "07195447", "04756076", "07196595", "07155686", "01238738", "00772032", "00069993" ;
  :wordnet_verb_synset "00775477", "00716789",  "02572443" .

:Disaster a owl:Class ;
  rdfs:subClassOf :EnvironmentalOrEcologicalEvent ;
  rdfs:label "Disaster"@en ;
  rdfs:comment "An Event (either natural or human-made) with 'serious disruption occurring over a short or long period of time that causes widespread human, material, economic or environmental loss which exceeds the ability of the affected [Agent], community or society to cope using its own resources' (https://en.wikipedia.org/w/index.php?title=Disaster&oldid=1013917618)."@en ;
  :wordnet_noun_synset "00218366", "07329438" .

:DistributionAndSupply a owl:Class ;
  rdfs:subClassOf :EventAndState ;
  rdfs:label "Distribution and Supply"@en ;
  rdfs:comment "Events related to giving out materials/Resources to Agents (typically Persons)."@en ;
  :wordnet_noun_synset "00809586", "01085001", "01085569" ;
  :wordnet_verb_synset "01381221", "02047080" .

:DivorceAndSeparation a owl:Class ;
  rdfs:subClassOf :LifeEvent, :LegalEvent, :Separation ;
  rdfs:label "Divorce and Separation"@en ;
  rdfs:comment "An event and condition indicating that two people have dissolved their relationship/Marriage."@en ;
  :wordnet_noun_synset "01203761", "00216181" ;
  :wordnet_verb_synset "02436167" .

:EatingAndDrinking a owl:Class ;
  rdfs:subClassOf :BodilyAct ;
  rdfs:label "Eating and Drinking"@en ;
  rdfs:comment "An activity related to an animal's or Person's intake of food/nutrients and/or liquids."@en ;
  :wordnet_noun_synset "00840028", "00839759" ;
  :wordnet_verb_synset "01168667", "01159300", "01203727" .

:EconomyAndFinanceRelated a owl:Class ;
  rdfs:subClassOf :EventAndState ;
  rdfs:label "Economy and Finance Related"@en ;
  rdfs:comment "Events dealing with monies/currencies, funds and other capital, as well as events related to the economy such as a change in taxes, becoming unemployed, etc."@en ;
  :wordnet_verb_synset "02222048", "02221793", "02220288", "02221492" .

:EducationEvent a owl:Class ;
  rdfs:subClassOf :EventAndState ;
  rdfs:label "Education Event"@en ;
  rdfs:comment "Events dealing with education and related learning activities such as science or book fairs, mentoring, classroom lessons, practice and drills, etc."@en ;
  :wordnet_noun_synset "00895653", "00884975" ;
  :wordnet_verb_synset "00604200", "00830768" .

:Election a owl:Class ;
  rdfs:subClassOf :PoliticalEvent ;
  rdfs:label "Election"@en ;
  rdfs:comment "The act of choosing an Agent to play a role or to hold a position within a GroupOfAgents."@en ;
  :example "Examples are the election of a Person to political office, or to serve in a role such as a jury foreman or chairman of a committee."@en ;
  :wordnet_noun_synset "00182630", "00184354", "00181811" ;
  :wordnet_verb_synset "02405902", "02466737" .

:EmotionalResponse a owl:Class ;
  rdfs:subClassOf :Cognition ;
  rdfs:label "Emotional Response"@en ;
  rdfs:comment "A state of mind associated with positive/pleasurable or negative/displeasurable feelings, thoughts and moods."@en ;
  :wordnet_noun_synset "00026390", "07495208", "11437243" ;
  :wordnet_verb_synset "00692071", "00719282" .

:Enforcement a owl:Class ;
  rdfs:subClassOf :EventAndState ;
  rdfs:label "Enforcement"@en ;
  rdfs:comment "An act that compels/insists on obedience or compliance to a law or obligation."@en ;
  :wordnet_noun_synset "01129340" ;
  :wordnet_verb_synset "02565990", "02566249" .

:EntranceAndExit a owl:Class ;
  rdfs:subClassOf :MovementTravelAndTransportation ;
  rdfs:label "Entrance and Exit"@en ;
  rdfs:comment "A movement of ."@en ;
  :wordnet_noun_synset "00049744", "00049115", "00043495", "00281976" ;
  :wordnet_verb_synset "02388582", "02019450", "02009962", "02011431" .

:EnvironmentAndCondition a owl:Class ;
  rdfs:subClassOf :EventAndState ;
  rdfs:label "Environment and Condition"@en ;
  rdfs:comment "A factor, situation or condition related to an Agent's (defined using the :has_holder property) or Resource's (defined using the :has_resource predicate) living conditions, external circumstances or physical environment at some time (defined using the :has_time property or its sub-properties) and place (defined using the :has_location property)."@en ;
  :example "For example, when hypothesizing about possible (or impossible), future scenarios, one can use a sub-class of EnvironmentAndCondition (OpportunityOrPossibility or Impossibility) to create this world/'environment'. Or, a sub-class (DrinkableWater) can describe that a Person or community lives in an area without potable water."@en ;
  :wordnet_noun_synset "13943868" .

:EnvironmentalOrEcologicalEvent a owl:Class ;
  rdfs:subClassOf :EventAndState ;
  rdfs:label "Environmental or Ecological Event"@en ;
  rdfs:comment "An occurrence in some geographic region that affects the natural world and the habitats of (and relationships between) plants and animals."@en ;
  :wordnet_verb_synset "00493642", "00493246" .

:FriendlyOrSupportiveAct a owl:Class ;
  rdfs:subClassOf :Agreement ;
  rdfs:label "Friendly or Supportive Act"@en ;
  rdfs:comment "Favorable, encouraging or helpful actions or statements. Note that if the Event involved a statement/communication, then the individual should also be classified as a :CommunicationAndSpeechAct."@en ;
  :wordnet_noun_synset "01216661", "01215009" ;
  :wordnet_verb_synset "00896689" .

:GamblingAndWagering a owl:Class ;
  rdfs:subClassOf :RiskTaking ;
  rdfs:label "Gambling and Wagering"@en ;
  rdfs:comment "An Event where an Agent takes a risk (or performs a risky action) in the hopes of success/reward/a desired result."@en ;
  :wordnet_noun_synset "00431125", "00491361", "00494042", "00494319", "00495779", "00492724" ;
  :wordnet_verb_synset "01140949", "02550045", "01079346" . 

:HealthAndDiseaseRelated a owl:Class ;
  rdfs:subClassOf :EventAndState ;
  rdfs:label "Health and Disease Related"@en ;
  rdfs:comment "Any event or condition concerning disease, disorders, illness, etc. (and recovery from such) by humans, plants and animals. Specific diseases, illnesses, etc. are subclasses."@en ;
  :wordnet_noun_synset "04081594", "00830651", "14075528" ; 
  :wordnet_verb_synset "00081478", "00086587" .

:ImitationAndCounterfeit a owl:Class ;
  rdfs:subClassOf :Substitution ;
  rdfs:label "Imitation and Counterfeit"@en ;
  rdfs:comment "An act of simulating or making a copy or duplicate of something or someone. If done to deceive, then this is counterfeiting."@en ;
  :wordnet_noun_synset "03109245" ;
  :wordnet_verb_synset "01657814", "01697776", "01740703" .

:ImpactAndContact a owl:Class ;
  rdfs:subClassOf :EventAndState ;
  rdfs:label "Impact and Contact"@en ;
  rdfs:comment "An act of coming into physical contact/touching, which may be forceful (e.g., an impact)"@en ;
  :wordnet_noun_synset "07316161", "07316568", "07353152", "00047263" ;
  :wordnet_verb_synset "01208316", "01208838" .

:InclusionAttachmentAndUnification a owl:Class ;
  rdfs:subClassOf :EventAndState ;
  rdfs:label "Inclusion, Attachment and Unification"@en ;
  rdfs:comment "An act of fastening, joining, grouping or bringing together, etc."@en ;
  :wordnet_noun_synset "00379793", "14441799", "00148415", "00380230", "01215372" ; 
  :wordnet_verb_synset "00193830", "01464634", "00187671", "00368338", "00244010", "01387824" . 

:Increase a owl:Class ;
  rdfs:subClassOf :Change ;
  rdfs:label "Increase"@en ;
  rdfs:comment "Indicates a growth/rise in the availability/count/amount of something or in the demeanor/behavior of an Agent. The pace of the Increase can be described using an associated instance of :AssessmentMeasurement (associated using the :has_measurement property)."@en ;
  :wordnet_noun_synset "00364086" ; 
  :wordnet_verb_synset "00156409", "00231172", "00153083" .

:IncrementalMovement a owl:Class ;
  rdfs:subClassOf :MovementTravelAndTransportation ;
  rdfs:label "Incremental Movement"@en ;
  rdfs:comment "Any act that changes the location of something by small amounts or makes small changes to the location of something, such as putting an object on a table, pouring a liquid into a container, etc. The Agent which places the thing(s) is specified using the :has_active_agent predicate, while the entity(ies) that are placed/moved are identified using the :has_topic property. The thing that 'receives' the entity(ies) that are moved is defined using :has_instrument."@en ;
  :wordnet_noun_synset "00403343", "01053255" ; 
  :wordnet_verb_synset "01446765", "01544249", "01857055", "01870596", "01524685", "01854282", "01450719" .

:IssuingAndPublishing a owl:Class ;
  rdfs:subClassOf :EventAndState ;
  rdfs:label "Issuing and Publishing"@en ;
  rdfs:comment "An act of issuing/releasing an InformationSource such as a book, article, newspaper, etc., a work of art or music, ..., or making an announcement/releasing a public statement."@en ;
  :wordnet_verb_synset "00956640" .

:LegalEvent a owl:Class ;
  rdfs:subClassOf :EventAndState ;
  rdfs:label "Legal Event"@en ;
  rdfs:comment "Any activity based on following legal practices, or related to or allowed by laws or the legal system."@en ;
  :wordnet_noun_synset "01183965", "01187304", "01183047", "01183348", "01183702", "01081986", "01204674", "08431076", "06660952", "01194465" ;
  :wordnet_verb_synset "02588535", "01016830", "02267740", "02503473", "00762621", "00896020", "00908688", "01015049" .

:LifeEvent a owl:Class ;
  rdfs:subClassOf :EventAndState ;
  rdfs:label "Life Event"@en ;
  rdfs:comment "Any occurrence in an Agent's existence, such as birth, death, marriage, etc."@en .

:Marriage a owl:Class ;
  rdfs:subClassOf :LifeEvent, :Ceremony, :PromiseAndOath, :LegalEvent ;
  rdfs:label "Marriage"@en ;
  rdfs:comment "A formal/legal event and condition describing that two people have committed to a relationship with each other."@en ;
  :wordnet_noun_synset "01038810", "01038935", "01039028" ; 
  :wordnet_verb_synset "02494483", "00888123" .

:MeetingAndEncounter a owl:Class ;
  rdfs:subClassOf :EventAndState ;
  rdfs:label "Meeting and Encounter"@en ;
  rdfs:comment "Any Event that is a formal, informal or coincidental gathering or assembly of people."@en ;
  :wordnet_noun_synset "00148007", "01232427" ; 
  :wordnet_verb_synset "02382049", "02026953" . 

:MovementTravelAndTransportation a owl:Class ;
  rdfs:subClassOf :EventAndState ;
  rdfs:label "Movement, Travel and Transportation"@en ;
  rdfs:comment "Any act that changes the location of something or someone. If movement is accomplished using a vehicle (such as an airplane, train, ship or truck), that mode of transport is indicated using the :has_instrument property. The Agent which moves the things or people is specified using the :has_active_agent predicate, while the entity that is moved is identified using the :has_topic property. And, to identify the Agents sending/receiving the entities or their origin/destination locations, the properties, :has_provider/recipient and :has_origin/destination (respectively), should be used."@en ;
  :wordnet_noun_synset "00280679" ;
  :wordnet_verb_synset "01839438", "00270891", "00415334", "01091334", "01438013", "01452567", "01517828", "01569697", "01954657", "01955339", "01957669", "02006752", "02060895", "02063390", "02236972" .

:NegativeEmotion a owl:Class ;
  rdfs:subClassOf :EmotionalResponse ;
  rdfs:label "Negative Emotion"@en ;
  rdfs:comment "Any EmotionalResponse related to unpleasant, pessimistic or insecure feelings."@en ;
  :example "Examples are unhappiness, fear, frustration, loneliness, disgust, hatred, etc., which are defined as subclasses"@en .

:PoliticalEvent a owl:Class ;
  rdfs:subClassOf :EventAndState ;
  rdfs:label "Political Event"@en ;
  rdfs:comment "Any Event related to the governance, government and public affairs of a community or country."@en ;
  :wordnet_noun_synset "01126829" .

:PositiveEmotion a owl:Class ;
  rdfs:subClassOf :EmotionalResponse ;
  rdfs:label "Positive Emotion"@en ;
  rdfs:comment "Any EmotionalResponse related to constructive, optimistic or confident feelings."@en ;
  :example "Examples are happiness, love, forgiveness, hope, gratitude, etc., which are defined as subclasses."@en ;
  :wordnet_noun_synset "04647533" .

:ProductionManufactureAndCreation a owl:Class ;
  rdfs:subClassOf :EventAndState ;
  rdfs:label "Production, Manufacture and Creation"@en ;
  rdfs:comment "Events involved with defining, supervising and engaging in the construction of some entity. The entity that is manufactured/created/produced is defined using the :has_topic predicate."@en ;
  :wordnet_noun_synset "00910607", "00942228", "03587827", "05641230", "00912746" ; 
  :wordnet_verb_synset "00094214", "01624592", "01660471", "01656984", "01635953" .

:Punishment a owl:Class ;
  rdfs:subClassOf :EventAndState ;
  rdfs:label "Punishment"@en ;
  rdfs:comment "An act of penalizing an Agent because of some occurrence/offense. The Event which is the (perceived) offense is identified using the :has_topic predicate. The Agent (e.g., an Animal, Person or GroupOfAgents) that is punished is indicated using the :has_affected_agent property. And, the details of the punishment are defined using the :has_instrument property."@en ;
  :wordnet_noun_synset "01162829" ; 
  :wordnet_verb_synset "00202809", "02505278" . 

:ReligionRelated a owl:Class ;
  rdfs:subClassOf :EventAndState ;
  rdfs:label "Religion Related"@en ;
  rdfs:comment "Any type of thing, activity, ceremony or condition related to faith, devotion and belief in a deity, or a higher meaning or consciousness. If the individual is a specific Ceremony, then also classify the instance using that type."@en ;
  :wordnet_noun_synset "01030024", "05793890", "01042678", "05955536" ;
  :wordnet_verb_synset "02619310" . 

:RemovalAndRestriction a owl:Class ;
  rdfs:subClassOf :EventAndState ;
  rdfs:label "Removal and Restriction"@en ;
  rdfs:comment "An act intended to decrease, reduce, take away, dispose of or discard something or someone. What is removed/restricted is identified using the :has_topic property. The thing or Agent that is affected by the removal/restriction is defined using the :has_affected_resource/:has_affected_agent properties (respectively)."@en ;
  :wordnet_noun_synset "00392407", "00809843", "01147872" ; 
  :wordnet_verb_synset "00173351", "00234091", "00450647" . 

:RemovalOfRawMaterials a owl:Class ;
  rdfs:subClassOf :RemovalAndRestriction ;
  rdfs:label "Removal of Raw Materials (Mining, Drilling, Logging, ...)"@en ;
  rdfs:comment "A removal or reduction in raw materials due to mining, logging, fishing, drilling and similar activities"@en ;
  :wordnet_noun_synset "00610057", "00924141", "00924782", "00582809", "00924944", "00944615" ;
  :wordnet_verb_synset "01165936", "01166163", "01313320", "01445640", "01261392" . 

:ReturnRecoveryAndRelease a owl:Class ;
  rdfs:subClassOf :EventAndState ;
  rdfs:label "Return, Recovery and Release"@en ;
  rdfs:comment "An act of restoring something or someone to their original owner/location/condition, granting freedom to someone or something, or publishing/releasing something. Note that the entity that is returned/released can be described using the :has_topic predicate, while the original (owning) Agent or location can be specified using the :has_affected_agent and :has_origin properties (respectively)."@en ;
  :wordnet_noun_synset "00046648", "07434392", "00096322", "00096791", "00214561", "00090171" ; 
  :wordnet_verb_synset "02557529", "02289796", "02426474", "02502711", "01477180" . 

:RewardAndCompensation a owl:Class ;
  rdfs:subClassOf :EventAndState ;
  rdfs:label "Reward and Compensation"@en ;
  rdfs:comment "An act of giving something or someone to an Agent to recognize their services, achievements/accomplishments or efforts. If a specific EventAndState (such as affiliation with an Organization) is being recognized, that is identified using the :has_topic predicate. The Agent (e.g., an Animal, Person or GroupOfAgents) that is rewarded is indicated using the :has_affected_agent property. And, the details of the reward are defined using the :has_instrument property."@en ;
  :wordnet_noun_synset "13304787", "06709228", "13303030" ;
  :wordnet_verb_synset "00789322", "02266695", "02551772" . 

:RiskTaking a owl:Class ;
  rdfs:subClassOf :EventAndState ;
  rdfs:label "Risk Taking"@en ;
  rdfs:comment "Proceeding with an act that is dangerous and/or may result in injury, failure or loss."@en ;
  rdfs:comment "Proceeding with an act that is dangerous and/or that has the 'possibility of something bad happening. Risk involves uncertainty about the effects/implications of an activity with respect to something that humans value (such as health, well-being, wealth, property or the environment), often focusing on negative, undesirable consequences. ... The understanding of risk, the methods of assessment and management, the descriptions of risk and even the definitions of risk differ in different practice areas (business, economics, environment, finance, information technology, health, insurance, safety, security etc).' (https://en.wikipedia.org/w/index.php?title=Risk&oldid=1013804959) It is expected that further subclasses will be defined to clarify the different understandings."@en ;
  :wordnet_noun_synset "00803899", "04669283", "04866016", "04867047" ; 
  :wordnet_verb_synset "02551275" . 

:Search a owl:Class ;
  rdfs:subClassOf :EventAndState ;
  rdfs:label "Search"@en ;
  rdfs:comment "An act of looking for something or someone. The entity that is searched for is identified using the :has_topic property."@en ;
  :wordnet_noun_synset "00453279", "00947217" ;
  :wordnet_verb_synset "01318273", "00790800", "01320383", "01146304", "02004900" .

:Separation a owl:Class ;
  rdfs:subClassOf :EventAndState ;
  rdfs:label "Separation"@en ;
  rdfs:comment "An act of moving two or more things or Agents some distance from each other, or of breaking an entity into its parts."@en ;
  :wordnet_noun_synset "14441101", "14440955", "08664696", "00386599" ; 
  :wordnet_verb_synset "00209582", "02036260", "00331375", "02035003", "00334996", "00369315", "00495205" . 

:SiegeAndSurrounding a owl:Class ;
  rdfs:subClassOf :RemovalAndRestriction ;
  rdfs:label "Siege and Surrounding"@en ;
  rdfs:comment "An act of encircling a Location."@en ;
  :wordnet_noun_synset "00956197" ; 
  :wordnet_verb_synset "01129272", "01129387", "01129837", "01133033", "01469999", "01571714", "01589983" . 

:SpaceEvent a owl:Class ;
  rdfs:subClassOf :EventAndState ;
  rdfs:label "Space Event"@en ;
  rdfs:comment "Any event that occurs beyond the Earth."@en ;
  :example "Examples are comet/asteroid/meteoroid observations and impacts, burn-up of space debris in the atmosphere, etc."@en ;
  :wordnet_noun_synset "09300592", "00293825", "00314328", "04272778", "04273014", "04273124", "04273272", "04273485", "07383246", "11527418" ;
  :wordnet_verb_synset "01517688", "01910195" . 

:StateAndPhysicalChange a owl:Class ;
  rdfs:subClassOf :Change ;
  rdfs:label "State Change and Physical Change"@en ;
  rdfs:comment "An Event indicating that some entity has been modified by the application of heat, cooling, pressure, human activity, etc. The entity that is affected is identified using the property, :has_topic."@en ;
  :wordnet_noun_synset "00405224", "00199979" ;
  :wordnet_verb_synset "00139943", "00140787", "00144670", "00145958", "00209244", "00238763", "00239753", "00255753", "00283693", "00313162" .

:Storage a owl:Class ;
  rdfs:subClassOf :EventAndState ;
  rdfs:label "Storage"@en ;
  rdfs:comment "Any act of keeping something for future delivery, sale or use."@en ;
  :wordnet_noun_synset "00373415", "04336084", "13389225", "08479216", "00813016" ; 
  :wordnet_verb_synset "02285938", "02287351", "02290237", "02208876" .  

:Substitution a owl:Class ;
  rdfs:subClassOf :EventAndState ;
  rdfs:label "Substitution"@en ;
  rdfs:comment "An act of replacing something or someone with another."@en ;
  :wordnet_noun_synset "00197334", "07458361" ; 
  :wordnet_verb_synset "02262575", "02263424" . 

:Suicide a owl:Class ;
  rdfs:subClassOf :Death ;
  rdfs:label "Suicide"@en ;
  rdfs:comment "The act of an individual (animal or Person) taking their own life."@en ;
  :wordnet_noun_synset "00223352", "10693108" ; 
  :wordnet_verb_synset "01327678" . 

:TechnologyRelated a owl:Class ;
  rdfs:subClassOf :EventAndState ;
  rdfs:label "Technology Related"@en ;
  rdfs:comment "An activity involved with understanding or using science and technology, involving computers, computer networks, and scientific devices and instruments. Included in this semantic is the collection, manipulation, protection or disruption of data/information. Note that the activities of protection and disruption are often referred to as 'cyber' activities."@en ;
  :wordnet_noun_synset "00103599", "13476660", "00643063", "00951435" ; 
  :wordnet_verb_synset "01751525" .  

:TransferOfPower a owl:Class ;
  rdfs:subClassOf :Change, :PoliticalEvent ;
  rdfs:label "Transfer of Governmental Power"@en ;
  rdfs:comment "Change of a government or government official. The Person or PoliticalParty who is out-going is identified using the :has_affected_agent property, while the new official/party is identified using :has_active_agent."@en .

:UtilizationAndConsumption a owl:Class ;
  rdfs:subClassOf :EventAndState ;
  rdfs:label "Utilization And Consumption"@en ;
  rdfs:comment "Any act that uses something or someone."@en ;
  :wordnet_noun_synset "00948944", "00357025" ; 
  :wordnet_verb_synset "01159815", "01167359", "01160888", "01161188" . 

:WeatherEvent a owl:Class ;
  rdfs:subClassOf :EnvironmentalOrEcologicalEvent ;
  rdfs:label "Weather Event"@en ;
  rdfs:comment "Any environmental occurrence related to atmospheric conditions in an area. If the event is also a Disaster, also add that class as a type."@en ;
  :wordnet_noun_synset "06763412", "11445694", "11482925" ;
  :wordnet_verb_synset "02762779", "00217578", "02775199", "02776493" . 


########################################################################
# Disjointness
########################################################################

[] rdf:type owl:AllDisjointClasses ;
  owl:members  ( :AggressiveCriminalOrHostileAct :FriendlyOrSupportiveAct ) .

[] rdf:type owl:AllDisjointClasses ;
  owl:members  ( :Agreement :DisagreementAndDispute ) .

[] rdf:type owl:AllDisjointClasses ;
  owl:members  ( :Cooperation :Competition ) .

[] rdf:type owl:AllDisjointClasses ;
  owl:members  ( :Decrease :Increase ) .

[] rdf:type owl:AllDisjointClasses ;
  owl:members  ( :DivorceAndSeparation :Marriage ) .

[] rdf:type owl:AllDisjointClasses ;
  owl:members  ( :InclusionAttachmentAndUnification :Separation ) .

[] rdf:type owl:AllDisjointClasses ;
  owl:members  ( :ProductionManufactureAndCreation :UtilizationAndConsumption ) .

[] rdf:type owl:AllDisjointClasses ;
  owl:members  ( :RemovalAndRestriction :ReturnRecoveryAndRelease ) .

[] rdf:type owl:AllDisjointClasses ;
  owl:members  ( :RewardAndCompensation :Punishment ) .


########################################################################
# Datatype Properties
########################################################################

:assessment a owl:DatatypeProperty, owl:FunctionalProperty ; 
  rdfs:subPropertyOf :reported_value ;
  rdfs:label "assessment"@en ;
  rdfs:comment "A restricted set of string values indicating how an AssessmentMeasurement for an entity (typically, a sub-class of EnvironmentAndCondition, such as Employment in a Country) is qualitatively evaluated - ranging from 'negligible or none' to 'very high'."@en ;
  rdfs:domain :AssessmentMeasurement ;
  rdfs:range [ a rdfs:Datatype ;
               owl:onDatatype xsd:string ;
               owl:oneOf  ('high' 'low' 'medium' 'negligible or none' 'very high' ) ] .

:reported_value a owl:DatatypeProperty, owl:FunctionalProperty ;
  rdfs:label "reported value"@en ;
  rdfs:comment "Specifies the value of a Measurement as a decimal (where the value's units are defined using the :has_unit predicate) or a string."@en ;
  rdfs:domain :Measurement ;
  rdfs:range [ a rdfs:Datatype ;
               owl:unionOf ( xsd:decimal xsd:string) ].


########################################################################
# Object Properties
########################################################################

:has_unit a owl:ObjectProperty, owl:FunctionalProperty ;
  rdfs:label "has unit of measure"@en ;
  rdfs:comment "Associates the units of a Measurement's :reported_value. Units are defined by QUDT.org and can be searched at http://www.qudt.org/doc/DOC_VOCAB-UNITS.html."@en ;
  rdfs:domain :Measurement ;
  rdfs:range <http://qudt.org/schema/qudt/Unit> .
