@prefix : <urn:ontoinsights:dna:> .
@prefix dna: <urn:ontoinsights:dna:> .
@prefix owl: <http://www.w3.org/2002/07/owl#> .
@prefix rdf: <http://www.w3.org/1999/02/22-rdf-syntax-ns#> .
@prefix rdfs: <http://www.w3.org/2000/01/rdf-schema#> .
@prefix xsd: <http://www.w3.org/2001/XMLSchema#> .

########################################################################
# File defining semantics related to events and states/conditions/situations
# 
# Created: February 9 2020
# Last modified: December 11 2024
# 
# Licensed by OntoInsights, LLC
# Creative Commons Attribution 4.0 International (CC BY 4.0)
# 
# Unless required by applicable law or agreed to in writing,
# software distributed under the License is distributed on an
# "AS IS" BASIS, WITHOUT WARRANTIES OR CONDITIONS OF ANY KIND,
# either express or implied.
# 
# Changes:
#  Reset change history and simplified, Nov 2023
#  Added :AchievementAndAccomplishment and :has_source
#  Separated :Win, :Loss
#  Added disjointess and :has_aspect
#  Removed :has_described_entity in lieu of :has_context, and 
#    :has_provider in lieu of :has_source
#  Changed range of :has_recipient to owl:Thing
#  Clarified several descriptions
########################################################################


########################################################################
# Classes
########################################################################

:AchievementAndAccomplishment a owl:Class ;
  rdfs:subClassOf :Success ;
  rdfs:label "Achievement and Accomplishment"@en ;
  rdfs:comment "The successful conclusion of an activity, where an achievement is more focused on the overall goal or purpose of the activity."@en ;
  :wordnet_noun_synset "00035910" ;
  :wordnet_verb_synset "02531751" .

:Continuation a owl:Class ;
  rdfs:subClassOf :EventAndState ;
  rdfs:label "Continuation"@en ;
  rdfs:comment "Indication that an ongoing EventAndState is still occurring - regardless of whether the actual time is known."@en ;
  :wordnet_noun_synset "01019929" ;
  :wordnet_verb_synset "00118331", "00783045" .

:End a owl:Class ;
  rdfs:subClassOf :EventAndState ;
  rdfs:label "End"@en ;
  rdfs:comment "The final point of an ongoing EventAndState - regardless of whether the actual end time is known."@en ;
  :wordnet_noun_synset "00210792" ;
  :wordnet_verb_synset "00353480" .

:Failure a owl:Class ;
  rdfs:subClassOf :End ;
  rdfs:label "Failure"@en ;
  rdfs:comment "A bad outcome or the inability to achieve a desired outcome - regardless of whether the actual failure details are known."@en ;
  :wordnet_noun_synset "00067036" ;
  :wordnet_verb_synset "02534046" .

:Loss a owl:Class ;
  rdfs:subClassOf :Failure ;
  rdfs:label "Loss"@en ;
  rdfs:comment "An outcome of some type of competition/engagement where an entity loses. The property, :has_active_entity defines the 'loser'."@en ;
  :wordnet_noun_synset "00068346" ;
  :wordnet_verb_synset "01102003" .

:Measurement a owl:Class ;
  rdfs:subClassOf :EventAndState ;
  rdfs:label "Measurement"@en ;
  rdfs:comment "The act of observing and reporting on properties such as length, size, amount, temperature, pressure, etc. at a specific time and location (as identified by the :has_time and :has_location properties). If the measurement is made by an instrument (such as a sensor), that can be specified using the :has_instrument property. The 'result' of a Measurement is indicated using the :reported_value property, and can be either a decimal or string value. The units of the Measurement are indicated using the :has_unit property."@en ;
  :wordnet_noun_synset "00998911" ; 
  :wordnet_verb_synset "00490773" . 

:StartAndBeginning a owl:Class ;
  rdfs:subClassOf :EventAndState ;
  rdfs:label "Start and Beginning"@en ;
  rdfs:comment "The originating point of an ongoing EventAndState - regardless of whether the actual start time is known."@en ;
  :wordnet_noun_synset "00236302" ;
  :wordnet_verb_synset "00346415", "00349400" .

:Success a owl:Class ;
  rdfs:subClassOf :End ;
  rdfs:label "Success"@en ;
  rdfs:comment "A good outcome or the accomplishment of an EventAndState - regardless of whether the actual success details are known."@en ;
  :wordnet_noun_synset "00064472", "00035910" ;
  :wordnet_verb_synset "02024442" .

:Win a owl:Class ;
  rdfs:subClassOf :Success ;
  rdfs:label "Win"@en ;
  rdfs:comment "An outcome of some type of competition/engagement where an entity is victorious/wins. Note that the property, :has_active_entity, defines the 'winner'."@en ;
  :wordnet_noun_synset "07369331" ;
  :wordnet_verb_synset "01102556" .


########################################################################
# Datatype Properties
########################################################################


########################################################################
# Object Properties
########################################################################

:has_active_entity a owl:ObjectProperty ;
  rdfs:label "has active entity"@en ;
  rdfs:domain :EventAndState ;
  rdfs:comment "References an entity who is an active/animate participant (carries out some action) in an EventAndState."@en .

:has_affected_entity a owl:ObjectProperty ;
  rdfs:label "has affected entity"@en ;
  rdfs:domain :EventAndState ;
  rdfs:comment "References an entity who is affected by an EventAndState, or experiences it, but does not actively participate in it."@en ;
  :example "For example, if a mob attacked a Person, then that event would be defined as an instance of an Attack (a subclass of EventAndState) where the mob (a GroupOfAgents) is referenced using the :has_active_entity property and the attacked Person is identified using the :has_affected_entity property."@en .

:has_aspect a owl:ObjectProperty ;
  rdfs:label "has aspect"@en ;
  rdfs:domain :EventAndState ;
  rdfs:comment "References the condition or an attribute of an entity, especially for an EnvironmentAndCondition event."@en .

:has_context a owl:ObjectProperty ;
  rdfs:label "has context"@en ;
  rdfs:domain :EventAndState ;
  rdfs:comment "References an entity which aids in the understanding of, and provides information on the circumstances or setting of an event or state."@en ;
  :example "For example, the general situation regarding the number of employed/unemployed individuals in a GeopoliticalEntity (such as a Country) would associate the Country to an Employment/Unemployment individual (subclass of EnvironmentAndCondition) using the property, :has_context. As examples ... if there is an investigation of a crime, then the crime would be some subclass of EventAndState (such as an AttackDamageAndAssault instance), and the Investigation event would reference that earlier attack/assualt using the :has_context property. And, if a farmer has a large fruit crop, that situation would be described using an instance of an :AgricultureApicultureAndAquacultureEvent with the :has_context property referencing the farmer (or his/her farm as a business/Organization) and the :has_topic property referencing the fruit (a sub-class of Resource -> FoodAndDrink)."@en .

:has_destination a owl:ObjectProperty ;
  rdfs:subPropertyOf :has_location ;
  rdfs:label "has destination"@en ;
  rdfs:domain :EventAndState ;
  rdfs:range :Location ;
  rdfs:comment "References the final location when an EventAndState involves movement of persons, goods, information, etc."@en .

:has_instrument a owl:ObjectProperty ;
  rdfs:label "has instrument"@en ;
  rdfs:domain :EventAndState ;
  rdfs:range :Resource ;
  rdfs:comment "References an inanimate entity (weapon, tool, etc.) that is/was used in an EventAndState."@en .

:has_origin a owl:ObjectProperty ;
  rdfs:subPropertyOf :has_location, :has_source ;
  rdfs:label "has origin"@en ;
  rdfs:domain :EventAndState ;
  rdfs:range :Location ;
  rdfs:comment "References the original location when an EventAndState involves movement of persons, goods, information, etc."@en .

:has_quantification  a owl:ObjectProperty ;
  rdfs:label "has quantification"@en ;
  rdfs:domain :EventAndState ;
  rdfs:range :Measurement ;
  rdfs:comment "References a statistic, assessment, time period, etc. pertaining to an EventAndState."@en .

:has_recipient a owl:ObjectProperty ;
  rdfs:label "has receiving agent"@en ;
  rdfs:domain :EventAndState ;
  rdfs:comment "References the entity that receives goods, information, ... when an EventAndState involves movement of persons, cargos, etc. or the application of medicine, chemicals, etc."@en .

:has_source a owl:ObjectProperty ;
  rdfs:label "has source"@en ;
  rdfs:domain :EventAndState ;
  rdfs:comment "References an entity in the semantic role of 'source'. That is the original location of something (which is refined as :has_origin), the entity from which a sensation or thought originates, the owner of something involved in a transfer, etc."@en .

:has_topic a owl:ObjectProperty ;
  rdfs:label "has topic"@en ;
  rdfs:domain :EventAndState ;
  rdfs:comment "References the subject/topic of an EventAndState."@en ;
  :example "For example, if a farmer has a large fruit crop that situation would be described using an instance of an :AgricultureApicultureAndAquacultureEvent with the :has_context property referencing the farmer (or his/her farm as a business/Organization) and the fruit (a sub-class of Resource -> FoodAndDrink) defined using the :has_topic property."@en .

:scheduled_time a owl:ObjectProperty ;
  rdfs:label "scheduled time"@en ;
  rdfs:subPropertyOf :has_time ;
  rdfs:domain :EventAndState ;
  rdfs:range :Time ;
  rdfs:comment "References a Time at which some event will/should occur or some condition should be in effect."@en .


########################################################################
# Disjointness
########################################################################

[] rdf:type owl:AllDisjointClasses ;
  owl:members  ( :StartAndBeginning :End ) .

[] rdf:type owl:AllDisjointClasses ;
  owl:members  ( :Success :Failure ) .

[] rdf:type owl:AllDisjointClasses ;
  owl:members  ( :Win :Loss ) .
