@prefix : <urn:ontoinsights:dna:> .
@prefix dna: <urn:ontoinsights:dna:> .
@prefix owl: <http://www.w3.org/2002/07/owl#> .
@prefix rdf: <http://www.w3.org/1999/02/22-rdf-syntax-ns#> .
@prefix rdfs: <http://www.w3.org/2000/01/rdf-schema#> .
@prefix xsd: <http://www.w3.org/2001/XMLSchema#> .

########################################################################
# File defining the properties and relationships of InformationSources
# and their graphs.
# 
# Created: October 31 2023
# Last modified: December 13 2024
# 
# Licensed by OntoInsights, LLC
# Creative Commons Attribution 4.0 International (CC BY 4.0)
# 
# Unless required by applicable law or agreed to in writing,
# software distributed under the License is distributed on an
# "AS IS" BASIS, WITHOUT WARRANTIES OR CONDITIONS OF ANY KIND,
# either express or implied.
# 
# Changes:
#  Added/clarified :number_sentences, :number_ingested and :rhetorical_device
#  Added :interpretation, :segment_level, :sentiment_explanation and :subject_area
#  Updated :text_quote to :partial_quote
#  Changed the domain of :rhetorical_device
#  Added :NarrativeEvent, :describes, :clarifying_text and :clarifying_reference
########################################################################


########################################################################
# Classes
########################################################################

:NarrativeEvent a owl:Class ;
  rdfs:subClassOf :EventAndState ;
  rdfs:label "Narrative Event"@en ;
  rdfs:comment "A main event or situation described in a Narrative. The NarrativeEvent is related to the Narrative using the :describes property. The :offset property indicates the ordering of the NarrativeEvents as they occur in the Narrative."@en .


########################################################################
# Datatype Properties
########################################################################

:author a owl:DatatypeProperty ;
  rdfs:label "author"@en ;
  rdfs:comment "String holding the author/creator of the InformationSource. There may be more than one."@en ;
  rdfs:domain :InformationSource ;
  rdfs:range xsd:string .

:clarifying_text a owl:DatatypeProperty ;
  rdfs:label "clarifying text"@en ;
  rdfs:comment "String holding the text of an adjective, preposition or possessive that clarifies the context of the entity."@en ;
  rdfs:range xsd:string .

:errors a owl:DatatypeProperty, owl:FunctionalProperty ;
  rdfs:label "errors (boolean)"@en ;
  rdfs:comment "Boolean indicating whether the referencing Sentence contains grammatical or spelling errors."@en ;
  rdfs:domain :Sentence ;
  rdfs:range xsd:boolean .

:grade_level a owl:DatatypeProperty, owl:FunctionalProperty ;
  rdfs:label "grade level"@en ;
  rdfs:comment "Defines the grade level of an individual who can understand the full semantics of the Sentence."@en ;
  rdfs:domain :Sentence ;
  rdfs:range xsd:integer .

:information_flow a owl:DatatypeProperty ;
  rdfs:label "information flow"@en ;
  rdfs:domain :Narrative ;
  rdfs:range [ a rdfs:Datatype ;
               owl:onDatatype xsd:string ;
               owl:oneOf  ('narrative/episodic' 'chronological' 'comparative' 'thematic/multifaceted' 'analytical'
                   'argumentative' 'causal' 'fragmented' 'speculative/forward-looking' 'historical context'
                   'cyclical' 'spiral' 'summarized' 'inverted pyramid' 'question-answer' ) ] ;
  rdfs:comment "String restricted to a set of values that indicate the possible flows of information in a narrative/article. Examples include 'episodic', 'argumentative' and 'summarized'."@en .

:interpretation a owl:DatatypeProperty ;
  rdfs:label "interpretation"@en ;
  rdfs:comment "Defines the emotional reaction expected of a reader with a certain viewpoint or perspective. The latter is specified using :segment_label as an edge property."@en ;
  rdfs:domain :Narrative ;
  rdfs:range xsd:string .

:narrative_goal a owl:DatatypeProperty ;
  rdfs:label "narrative goal"@en ;
  rdfs:domain :Narrative ;
  rdfs:range [ a rdfs:Datatype ;
               owl:onDatatype xsd:string ;
               owl:oneOf  ('advocate' 'analyze' 'describe-set' 'describe-current' 'entertain'
                           'establish-authority' 'inspire' 'life-story' ) ] ;
  rdfs:comment "String restricted to a set of values that indicate the possible purposes/goals for publishing a narrative. There are many possible goals that may apply to a single Narrative. As an example, values include 'advocate'ing, 'analyze'ing and 'entertain'ing."@en .

:narrative_plotline a owl:DatatypeProperty ;
  rdfs:label "narrative plotline"@en ;
  rdfs:domain :Narrative ;
  rdfs:range [ a rdfs:Datatype ;
               owl:onDatatype xsd:string ;
               owl:oneOf  ('conflict and resolution' 'rise and fall' 'overcoming the monster/heroic acts' 'rags to riches'
                           'scandal and accountability' 'quest' 'personal transformation' 'justice and revenge' ) ] ;
  rdfs:comment "String restricted to a set of values that indicate archetypal story themes/plotlines tied to human experiences and desires, that may be used in a narrative/article. There are many possible plotlines that may apply to a single Narrative. As an example, values include 'conflict and resolution', 'scandal and accountability' and 'rags to riches'."@en .

:number_characters a owl:DatatypeProperty, owl:FunctionalProperty ;
  rdfs:subPropertyOf :count ;
  rdfs:label "number of characters"@en ;
  rdfs:comment "Integer indicating the length (in characters) of the narrative/news article."@en ;
  rdfs:domain :Narrative ;
  rdfs:range xsd:integer .

:number_ingested a owl:DatatypeProperty, owl:FunctionalProperty ;
  rdfs:subPropertyOf :count ;
  rdfs:label "number of sentences ingested"@en ;
  rdfs:comment "A count of the number of sentences from an InformationSource that were fully ingested (with complete event detail processing)."@en ;
  rdfs:domain :InformationSource ;
  rdfs:range xsd:integer .

:number_sentences a owl:DatatypeProperty, owl:FunctionalProperty ;
  rdfs:subPropertyOf :count ;
  rdfs:label "number of sentences"@en ;
  rdfs:comment "A count of the number of sentences in an InformationSource."@en ;
  rdfs:domain :InformationSource ;
  rdfs:range xsd:integer .

:number_triples a owl:DatatypeProperty, owl:FunctionalProperty ;
  rdfs:subPropertyOf :count ;
  rdfs:label "number of triples"@en ;
  rdfs:comment "A count of the number of triples in an InformationGraph."@en ;
  rdfs:domain :InformationGraph ;
  rdfs:range xsd:integer .

:offset a owl:DatatypeProperty, owl:FunctionalProperty ;
  rdfs:label "offset"@en ;
  rdfs:comment "Defines the (incremental) Sentence number extracted from a Narrative."@en ;
  rdfs:domain :Sentence ;
  rdfs:range xsd:integer .

:partial_quote a owl:DatatypeProperty ;
  rdfs:subPropertyOf :text ;
  rdfs:label "partial quote"@en ;
  rdfs:comment "String holding the text of a short quotation (a few words without a subject and verb) in a Sentence."@en ;
  rdfs:domain :Sentence ;
  rdfs:range xsd:string .

:ranking a owl:DatatypeProperty ;
  rdfs:label "ranking"@en ;
  rdfs:comment "Defines a Narrative's validity as considered by a reader with a certain viewpoint or perspective. The latter is specified using :segment_label as an edge property. The ranking is an integer from 1 to 5, where 1 indicates that the Narrative is not considered valid/truthful."@en ;
  rdfs:domain :Narrative ;
  rdfs:range xsd:integer .

:rhetorical_device a owl:DatatypeProperty ;
  rdfs:label "rhetorical device"@en ;
  rdfs:domain :Sentence ;
  rdfs:range [ a rdfs:Datatype ;
               owl:onDatatype xsd:string ;
               owl:oneOf  ('ad baculum' 'ad hominem' 'ad populum' 'allusion' 'antanagoge' 'aphorism' 'ethos' 'exceptionalism' 
                           'expletive' 'hyperbole' 'imagery' 'invective' 'irony' 'juxtaposition' 'kairos' 'litote' 
                           'loaded language' 'logos' 'metaphor' 'nostalgia' 'paralipsis' 'pathos' 'pleonasm' 'repetition' 
                           'rhetorical question') ] ;
  rdfs:comment "String restricted to a set of values that indicate the rhetorical devices that are observed in a Sentence or Narrative. There are many possible devices that may be employed in an entity. As an example, values include 'allusion', 'loaded language' and 'nostalgia'."@en .

:segment_label a owl:DatatypeProperty, owl:FunctionalProperty ;
  rdfs:label "segment label"@en ;
  rdfs:comment "String specifying the perspective/viewpoint for interpreting a Narrative. This is an edge property on the :interpretation string property."@en ;
  rdfs:range xsd:string .

:sentence_person a owl:DatatypeProperty, owl:FunctionalProperty ;
  rdfs:label "sentence person"@en ;
  rdfs:comment "Defines the perspective/person of the Sentence - 1 for first person(I/we), 2 for second person (you) and 3 for third person (he/she/it/they)."@en ;
  rdfs:domain :Sentence ;
  rdfs:range xsd:integer .

:sentiment a owl:DatatypeProperty, owl:FunctionalProperty ;
  rdfs:label "sentiment"@en ;
  rdfs:domain :Narrative ;
  rdfs:range [ a rdfs:Datatype ;
               owl:onDatatype xsd:string ;
               owl:oneOf ( 'negative' 'neutral' 'positive' ) ] ;
  rdfs:comment "String restricted to a set of values that indicate whether a Narrative conveys a 'positive', 'negative' or 'neutral' sentiment."@en .

:sentiment_explanation a owl:DatatypeProperty, owl:FunctionalProperty ;
  rdfs:label "sentiment explanation"@en ;
  rdfs:domain :Narrative ;
  rdfs:range xsd:string ;
  rdfs:comment "String explaining why a sentiment of 'positive', 'negative' or 'neutral' was assigned to a Narrative."@en .
  
:source a owl:DatatypeProperty ;
  rdfs:label "source"@en ;
  rdfs:comment "String indicates the agent, location or means by which the InformationSource was obtained."@en ;
  rdfs:domain :InformationSource ;
  rdfs:range xsd:string .

:subject_area a owl:DatatypeProperty ;
  rdfs:label "subject area"@en ;
  rdfs:domain :Narrative ;
  rdfs:range [ a rdfs:Datatype ;
               owl:onDatatype xsd:string ;
               owl:oneOf  ( 'crime/law' 'economy/business' 'education' 'entertainment' 'environment/ecology' 'health' 
                            'lifestyle' 'politics/international' 'science/technology' 'sports' ) ] ;
  rdfs:comment "String restricted to a set of values that indicate the subject areas that describe a Narrative. As an example, values include 'crime/law', 'health' and 'politics'."@en .

:summary a owl:DatatypeProperty, owl:FunctionalProperty ;
  rdfs:label "summary"@en ;
  rdfs:comment "Provides a short summarization of a Sentence or Narrative."@en ;
  rdfs:domain [ a owl:Class ;
                owl:unionOf ( :Narrative :Sentence ) ] ;
  rdfs:range xsd:string .

:tense a owl:DatatypeProperty, owl:FunctionalProperty ;
  rdfs:label "tense"@en ;
  rdfs:comment "Defines the whether a Sentence is written in the 'past', 'present' or 'future' tense."@en ;
  rdfs:domain :Sentence ;
  rdfs:range [ a rdfs:Datatype ;
               owl:onDatatype xsd:string ;
               owl:oneOf  ('neutral' 'past' 'present') ] .

:text a owl:DatatypeProperty, owl:FunctionalProperty ;
  rdfs:label "text"@en ;
  rdfs:comment "String holding the text of an InformationSource."@en ;
  rdfs:domain :InformationSource ;
  rdfs:range xsd:string .

:topic a owl:DatatypeProperty ;
  rdfs:label "topic"@en ;
  rdfs:comment "String holding a topic of the InformationSource."@en ;
  rdfs:domain :InformationSource ;
  rdfs:range xsd:string .
  
:voice a owl:DatatypeProperty, owl:FunctionalProperty ;
  rdfs:label "voice"@en ;
  rdfs:comment "Defines the whether a Sentence is written in the first, second or third person."@en ;
  rdfs:domain :Sentence ;
  rdfs:range [ a rdfs:Datatype ;
               owl:onDatatype xsd:integer ;
               owl:withRestrictions ( [ xsd:minInclusive "1"^^xsd:integer ]
                                      [ xsd:maxInclusive "3"^^xsd:integer ] ) ] .


########################################################################
# Object Properties
########################################################################

:attributed_to a owl:ObjectProperty, owl:FunctionalProperty ;
  rdfs:label "attributed to"@en ;
  rdfs:comment "Relationship between a Quote and the Agent to whom/which it is attributed."@en ;
  rdfs:domain :Quote ;
  rdfs:range :Agent .

:clarifying_reference a owl:ObjectProperty, owl:FunctionalProperty ;
  rdfs:label "clarifying reference"@en ;
  rdfs:comment "Relationship from an entity to another, typically indicating that the subject is part of or owned by the object, or that the object provides the context for the subject. The :clarifying_text indicates the string that was analyzed to determine the :clarifying_reference."@en .

:describes a owl:ObjectProperty ;
  rdfs:label "describes"@en ;
  rdfs:comment "Relationship between a Narrative and the main events/situations detailed in it."@en ;
  rdfs:domain :Narrative ;
  rdfs:range :NarrativeEvent .

:has_semantic a owl:ObjectProperty ;
  rdfs:label "has semantic"@en ;
  rdfs:comment "Relationship between a Sentence and the events and/or conditions detailed in it."@en ;
  rdfs:domain :Sentence ;
  rdfs:range :EventAndState .

:mentions a owl:ObjectProperty ;
  rdfs:label "mentions"@en ;
  rdfs:domain :Sentence ;
  rdfs:comment "Indicates that the Sentence includes a reference to a specific named entity such as an agent (organization, person, etc.), time period or specific date/time, historical event (for example, World War II) or location."@en .
