@prefix : <urn:ontoinsights:dna:> .
@prefix dna: <urn:ontoinsights:dna:> .
@prefix owl: <http://www.w3.org/2002/07/owl#> .
@prefix rdf: <http://www.w3.org/1999/02/22-rdf-syntax-ns#> .
@prefix rdfs: <http://www.w3.org/2000/01/rdf-schema#> .
@prefix xsd: <http://www.w3.org/2001/XMLSchema#> .

########################################################################
# File defining semantics related to location 
# Many concepts are inspired by the GeoNames Feature Classes and 
# Codes (https://www.geonames.org/export/codes.html).
# 
# Created: February 9, 2020
# Last modified: October 31 2023
# 
# Licensed by OntoInsights, LLC
# Creative Commons Attribution 4.0 International (CC BY 4.0)
# 
# Unless required by applicable law or agreed to in writing,
# software distributed under the License is distributed on an
# "AS IS" BASIS, WITHOUT WARRANTIES OR CONDITIONS OF ANY KIND,
# either express or implied.
# 
# Changes:
#  Reset change history and simplified
########################################################################


########################################################################
# Classes
########################################################################

:AdministrativeDivision a owl:Class ;
  rdfs:subClassOf :GeopoliticalEntity ;
  rdfs:label "Administrative Division"@en ;
  rdfs:comment "A subnational level of government, operating over some region. The first-order administrative division is typically a state or province, but may be a territory or even a 'parish' in a smaller country. Other levels are defined below the first-order division - such as counties within states, districts within provinces, etc. The level of an AdministrativeDivision is given by the property, :admin_level. Note that :admin_level is an optional property and may not be known, or applicable."@en ;
  :wordnet_noun_synset "08508836" .

:AnthropogenicFeature a owl:Class ;
  rdfs:subClassOf :PhysicalLocation ;
  rdfs:label "Anthropogenic (Human-Created) Feature"@en ;
  rdfs:comment "A point or site on/in the Earth which is a human-created structure that is used for a particular industry or purpose. The specific location is identified by latitude/longitude/altitude, by name or street address, or by nearby points and sites."@en .

:BoundingRegion a owl:Class ;
  rdfs:subClassOf :PhysicalLocation ;
  rdfs:label "Bounding Region"@en ;
  rdfs:comment "A BoundingRegion is defined by at least three sets of latitude/longitude coordinates (instances of PhysicalLocation with :latitude/longitude properties) which enclose the region. The PhysicalLocations that define the points are referenced using the :has_bounding_coordinate property."@en ;
  :wordnet_noun_synset "08647614" .

:BuildingAndDwelling a owl:Class ;
  rdfs:subClassOf :AnthropogenicFeature, :Resource ;
  rdfs:label "Building and Dwelling"@en ;
  rdfs:comment "A physical structure that usually is located in a single place, with a roof, walls, door(s) and (possibly) windows and other details. The specific location is identified by latitude/longitude/altitude, by name or street address, or by nearby points and sites."@en ;
  :wordnet_noun_synset "02916498", "03264208", "02918337", "03745009", "02729230" .

:Continent a owl:Class ;
  rdfs:subClassOf :PhysicalLocation ;
  rdfs:label "Continent"@en ;
  rdfs:comment "One of the 7 large landmasses (Africa, Antarctica, Asia, Australia, Europe, North America, South America). The continents are instantiated using their GeoName idenfitiers in the file, geonames_countries.ttl."@en .

:Country a owl:Class ;
  rdfs:subClassOf :GeopoliticalEntity ;
  rdfs:label "Country"@en ;
  rdfs:comment "Describes the government of a nation, the people living in the nation and the land area that is governed."@en ;
  :wordnet_noun_synset "08185877" .

:Currency a owl:Class ;
  rdfs:subClassOf :MonetaryAndFinancialInstrument ;
  rdfs:label "Currency"@en ;
  rdfs:comment "A metal or paper medium of exchange that is used as money in a country."@en ;
  :wordnet_noun_synset "13407086" .

:DesignatedArea a owl:Class ;
  rdfs:subClassOf :PhysicalLocation ;
  rdfs:label "Designated Area"@en ;
  rdfs:comment "A portion of land identified for specific use."@en .

:Factory a owl:Class ;
  rdfs:subClassOf :BuildingAndDwelling ;
  rdfs:label "Factory"@en ;
  rdfs:comment "One or more buildings where goods are made, assembled, etc. which is accomplished by human labor and/or machines."@en ;
  :wordnet_noun_synset "03321351" .

:GeographicFeature a owl:Class ;
  rdfs:subClassOf :PhysicalLocation ;
  rdfs:label "Geographic Feature"@en ;
  rdfs:comment "Any type of physical feature associated with the geography of an area, such as a forest, monument, school campus, etc."@en .

:GeopoliticalEntity a owl:Class ;
  rdfs:subClassOf :Agent, :PhysicalLocation ;
  rdfs:label "Geopolitical Entity"@en ;
  rdfs:comment "A point or site on/in the Earth, related to a political entity (such as a country or city), as identified by latitude/longitude/altitude, by name or street address, or by nearby points and sites. Note that GeopoliticalEntity is defined as both a PhysicalLocation and an Agent. This is due to its usage in text and conversation."@en ;
  :example "For example, one may say 'California is in the western United States, and is considered to be quite liberal.' In that sentence, California is both a location, and an entity (Agent) that has a political orientation. Distinguishing the difference between these semantics is quite difficult, and usually unnecessary."@en .

:OccupiedArea a owl:Class ;
  rdfs:subClassOf :GeopoliticalEntity ;
  rdfs:label "Occupied Area"@en ;
  rdfs:comment "The land and government of a region which has been taken over/'occupied' by another nation/GPE."@en .

:OnlineLocation a owl:Class ;
  rdfs:subClassOf :Location ;
  rdfs:label "Online Location"@en ;
  rdfs:comment "A location defined in/on a network, such as a wireless network (e.g., a mobile phone number), the Internet (such an IP address, email adress or URL) or a wired network. The properties that define OnlineLocations include :url, :email_address, :ip_v4_address and :phone_number, among others."@en ;
  :wordnet_noun_synset "06367922" .

:PhysicalLocation a owl:Class ;
  rdfs:subClassOf :Location ;
  rdfs:label "Physical Location"@en ;
  rdfs:comment "A point or site on/in the Earth as identified by latitude/longitude/altitude, by name or street address, or by nearby points and sites."@en ;
  :wordnet_noun_synset "00027365" .

:PopulatedPlace a owl:Class ;
  rdfs:subClassOf :PhysicalLocation ;
  rdfs:label "Populated Place"@en ;
  rdfs:comment "A city, town, village, etc. where people live and work. The location is identified by latitude/longitude/altitude, by name or street address, or by nearby points and sites."@en .

:PostalAddress a owl:Class ;
  rdfs:subClassOf :PhysicalLocation ;
  rdfs:label "Postal Address"@en ;
  rdfs:comment "A point or site on/in the Earth as specified by a numeric identifier and street name or a post office box, along with other details such as a part of a city, a town/city name, state or other country locality information, country name and postal code. The details of a PostalAddress are defined using the properties, :street_address1, :street_address2, :city_part_name, :city_name, :state_or_region_name, :country_name and :postal_code, assembled in that order into a complete postal address. Note that all properties do NOT have to be specified."@en ;
  :wordnet_noun_synset "08508037" .

:RelativeDirectionLocation a owl:Class ;
  rdfs:subClassOf :PhysicalLocation ;
  rdfs:label "Relative Direction Location"@en ;
  rdfs:comment "A point or site on/in the Earth defined relative to another, 'established' Location. The 'established' location is referenced using the :near property. The distance from the 'established' Location is defined using the property, :distance_meters (or one of its sub-properties if an exact distance is not known). The direction from the 'established' :Location is specified using the :direction property. Any of the properties can be omitted if not known or not applicable."@en ;
  :wordnet_noun_synset "08578618", "08578767", "08578888", "08578999", "08579120", "08579251", "08579372", "08579483", "13852504" .

:TransportationFeature a owl:Class ;
  rdfs:subClassOf :AnthropogenicFeature ;
  rdfs:label "Transportation Feature"@en ;
  rdfs:comment "A point or site on/in the Earth related to roads, paths, etc. and related locations. The specific location is identified by latitude/longitude/altitude, by name or street address, or by nearby points and sites."@en ;
  :wordnet_noun_synset "08651532", "02690680", "02695091", "04055680", "04471218", "04056210", "04505257", "03610935", "02688444", "02929672", "04056210", "04356155", "02690680", "03221531", "00491580" .

:WaterFeature a owl:Class ;
  rdfs:subClassOf :PhysicalLocation ;
  rdfs:label "Water Feature"@en ;
  rdfs:comment "A body of water as identified by latitude/longitude/altitude, by name or street address, or by nearby points and sites."@en ;
  :wordnet_noun_synset "09248053", "03009709" .


########################################################################
# Datatype Properties
########################################################################

:admin_level a owl:DatatypeProperty, owl:FunctionalProperty ;
  rdfs:label "administrative level (1-5)"@en ;
  rdfs:comment "Integer (1-5) indicating a first-, second-, third-, fourth- or fifth-order administrative division."@en ;
  :example "A first-order administrative division is typically a state or province, but may be a territory or even a 'parish' in a small country. Other levels are defined below the first-order division - such as counties within states, districts within provinces, etc."@en ;
  rdfs:domain :AdministrativeDivision ;
  rdfs:range [ a rdfs:Datatype ;
               owl:onDatatype xsd:integer ;
               owl:withRestrictions ( [ xsd:minInclusive "1"^^xsd:integer ]
                                      [ xsd:maxInclusive "5"^^xsd:integer ] ) ] .

:altitude_meters a owl:DatatypeProperty ;
  rdfs:label "altitude in meters"@en ;
  rdfs:comment "A height (estimated) in meters, relative to sea level."@en ;
  rdfs:domain :PhysicalLocation ;
  rdfs:range xsd:decimal .

:city_name a owl:DatatypeProperty, owl:FunctionalProperty ;
  rdfs:subPropertyOf :postal_address_detail ;
  rdfs:label "city name"@en ;
  rdfs:comment "Identification of the city/town for a PopulatedPlace or that is a part of a PostalAddress."@en ;
  rdfs:domain [ a owl:Class ;
                owl:unionOf ( :PostalAddress :PopulatedPlace ) ] ; 
  rdfs:range xsd:string .

:city_part_name a owl:DatatypeProperty, owl:FunctionalProperty ;
  rdfs:subPropertyOf :postal_address_detail ;
  rdfs:label "name of a part of the city"@en ;
  rdfs:comment "A part of a PostalAddress identifying a particular part of a city or town."@en ;
  rdfs:domain :PostalAddress ;
  rdfs:range xsd:string .

:country_name a owl:DatatypeProperty, owl:FunctionalProperty ;
  rdfs:subPropertyOf :postal_address_detail ;
  rdfs:label "country name"@en ;
  rdfs:comment "Identification of the country for a PopulatedPlace or that is a part of a PostalAddress."@en ;
  rdfs:domain [ a owl:Class ;
                owl:unionOf ( :PostalAddress :PopulatedPlace ) ] ; 
  rdfs:range xsd:string .

:direction a owl:DatatypeProperty, owl:FunctionalProperty ;
  rdfs:label "direction"@en ;
  rdfs:comment "A restricted set of strings defining a compass direction. The values are 'north', 'south', 'east', 'west' and combinations (such as 'northeast')."@en ;
  rdfs:domain :RelativeDirectionLocation ;
  rdfs:range [ a rdfs:Datatype ;
               owl:onDatatype xsd:string ;
               owl:oneOf  ('east' 'north' 'northeast' 'northwest' 'south' 'southeast' 'southwest' 'west' ) ] .

:distance_meters a owl:DatatypeProperty, owl:FunctionalProperty ;
  rdfs:label "distance in meters"@en ;
  rdfs:comment "An (estimated) amount of space between entities, in meters."@en ;
  rdfs:domain :RelativeDirectionLocation ;
  rdfs:range xsd:decimal .

:email_address a owl:DatatypeProperty ;
  rdfs:label "email address"@en ;
  rdfs:comment "A unique identifier for an account on an email communications system."@en ;
  rdfs:domain :OnlineLocation ;
  rdfs:range [ a rdfs:Datatype ;
               owl:onDatatype xsd:string ;
               owl:withRestrictions ( [ xsd:pattern "^([^@\\.].*@.*[^@\\.])$" ] ) ] .

:ip_v4_address a owl:DatatypeProperty ;
  rdfs:label "IP V4 address"@en ;
  rdfs:comment "A string defining an OnlineLocation using a IPV4 address in dotted decimal format (e.g., 169.23.24.00)."@en ;
  rdfs:domain :OnlineLocation ;
  rdfs:range [ a rdfs:Datatype ;
               owl:onDatatype xsd:string ;
               owl:withRestrictions ( [ xsd:pattern "^(([0-9]|[1-9][0-9]|1[0-9]{2}|2[0-4][0-9]|25[0-5])\\.){3}([0-9]|[1-9][0-9]|1[0-9]{2}|2[0-4][0-9]|25[0-5])$" ] ) ] .

:ip_v6_address a owl:DatatypeProperty ;
  rdfs:label "IP V6 address"@en ;
  rdfs:comment "A string defining an OnlineLocation as an IPV6 address using hexadecimals (e.g., ffff:ffff:ffff:ffff:ffff:ffff:ffff:ffff)."@en ;
  rdfs:domain :OnlineLocation ;
  rdfs:range [ a rdfs:Datatype ;
               owl:onDatatype xsd:string ;
               owl:withRestrictions ( [ xsd:pattern "^([A-Fa-f0-9]{4}:|0:|:){7}([A-Fa-f0-9]{4}|0)$" ] ) ] .

:iso_alpha2 a owl:DatatypeProperty, owl:FunctionalProperty ;
  rdfs:label "ISO 2-character alpha code"@en ;
  rdfs:comment "A string specifying the 2 character ISO 3166 code of a country."@en ;
  rdfs:domain :Country ;
  rdfs:range [ a rdfs:Datatype ;
               owl:onDatatype xsd:string ;
               owl:withRestrictions ( [ xsd:pattern "^[A-Z]{2}$" ] ) ] .

:iso_alpha3 a owl:DatatypeProperty, owl:FunctionalProperty ;
  rdfs:label "ISO 3-character alpha code"@en ;
  rdfs:comment "A string specifying the 3 character ISO 3166 code of a country."@en ;
  rdfs:domain :Country ;
  rdfs:range [ a rdfs:Datatype ;
               owl:onDatatype xsd:string ;
               owl:withRestrictions ( [ xsd:pattern "^[A-Z]{3}$" ] ) ] .

:latitude a owl:DatatypeProperty, owl:FunctionalProperty ;
  rdfs:label "latitude"@en ;
  rdfs:comment "The angular distance north or south of the equator. Latitude is specified in decimal degrees."@en ;
  rdfs:domain :PhysicalLocation ;
  rdfs:range xsd:decimal .

:longitude a owl:DatatypeProperty, owl:FunctionalProperty ;
  rdfs:label "longitude"@en ;
  rdfs:comment "The angular distance east or west of the prime meridian at Greenwich, England. Longitude is specified in decimal degrees."@en ;
  rdfs:domain :PhysicalLocation ;
  rdfs:range xsd:decimal .

:phone_number a owl:DatatypeProperty ;
  rdfs:label "phone number"@en ;
  rdfs:comment "A string of numbers and/or letters identifying a telephone or mobile phone. A country code may be specified, as well as an extension number."@en ;
  :example "For example, using 44 as the country code for the United Kingdom, a phone_number may appear as '+44 (0) 5555-5555 x 1234'."@en ;
  rdfs:domain :OnlineLocation ;
  rdfs:range [ a rdfs:Datatype ;
               owl:onDatatype xsd:string ;
               owl:withRestrictions ( [ xsd:pattern "^(\\(?\\+?[0-9]*\\)?)?[ \\.\\-])?(\\(?[0-9]*\\)?)?[0-9A-Z \\.\\-\\(\\)]*((x|ext|extension)? ?[0-9]*)?$" ] ) ] .

:postal_address_detail a owl:DatatypeProperty ;
  rdfs:label "postal address detail"@en ;
  rdfs:comment "A property whose subproperties specify all the parts of a PostalAddress. The subproperties are :street_address1/2, :city_part_name, :city_name, :state_or_region_name, :country_name and :postal_code."@en ;
  rdfs:domain :PostalAddress ;
  rdfs:range xsd:string .

:postal_code a owl:DatatypeProperty, owl:FunctionalProperty ;
  rdfs:subPropertyOf :postal_address_detail ;
  rdfs:label "postal code"@en ;
  rdfs:comment "A part of a PostalAddress identifying a section of a city, state or country consisting of a group of numbers and/or letters, used to aid in the sorting of mail."@en ;
  rdfs:domain :PostalAddress ;
  rdfs:range xsd:string .

:state_or_region_name a owl:DatatypeProperty, owl:FunctionalProperty ;
  rdfs:subPropertyOf :postal_address_detail ;
  rdfs:label "state, province or region name"@en ;
  rdfs:comment "Identification of a first order administrative region, such as a state, province or district of a countrty for a PopulatedPlace or a part of a PostalAddress."@en ;
  rdfs:domain [ a owl:Class ;
                owl:unionOf ( :PostalAddress :PopulatedPlace ) ] ; 
  rdfs:range xsd:string .

:street_address1 a owl:DatatypeProperty, owl:FunctionalProperty ;
  rdfs:subPropertyOf :postal_address_detail ;
  rdfs:label "street address, line 1"@en ;
  rdfs:comment "A part of a PostalAddress specifying a house number and street name, post office box information or similar information."@en ;
  rdfs:domain :PostalAddress ;
  rdfs:range xsd:string .

:street_address2 a owl:DatatypeProperty, owl:FunctionalProperty ;
  rdfs:subPropertyOf :postal_address_detail ;
  rdfs:label "street address, line 2"@en ;
  rdfs:comment "A part of a Postal Address further clarifying the information in :street_address1."@en ;
  rdfs:domain :PostalAddress ;
  rdfs:range xsd:string .

:url a owl:DatatypeProperty ;
  rdfs:label "Uniform Resource Locator (URL)"@en ;
  rdfs:comment "A string defining a web address, using the HTTP or HTTPS protocols."@en ;
  rdfs:domain :OnlineLocation ;
  rdfs:range xsd:string .


########################################################################
# Object Properties
########################################################################

:has_bounding_coordinate a owl:ObjectProperty ;
  rdfs:subPropertyOf :has_location ;
  rdfs:label "has bounding coordinate"@en ;
  rdfs:comment "References a PhysicalLocation (specifying latitude/longitude properties) that defines one of at least three points of a BoundingRegion."@en ;
  rdfs:domain :BoundingRegion ;
  rdfs:range :PhysicalLocation .

:has_currency a owl:ObjectProperty, owl:FunctionalProperty ;
  rdfs:label "has currency"@en ;
  rdfs:comment "References the currency unit of a Country."@en ;
  rdfs:domain :Country ;
  rdfs:range :Currency .

:near a owl:ObjectProperty ;
  rdfs:label "near", "close"@en ;
  rdfs:comment "Indicates that a RelativeDirectionLocation is 'close to' another, 'established' PhysicalLocation."@en ;
  rdfs:domain :RelativeDirectionLocation ;
  rdfs:range :PhysicalLocation .
