@prefix : <urn:ontoinsights:dna:> .
@prefix dna: <urn:ontoinsights:dna:> .
@prefix owl: <http://www.w3.org/2002/07/owl#> .
@prefix rdf: <http://www.w3.org/1999/02/22-rdf-syntax-ns#> .
@prefix rdfs: <http://www.w3.org/2000/01/rdf-schema#> .
@prefix xsd: <http://www.w3.org/2001/XMLSchema#> .

########################################################################
# File defining semantics related to a variety of events that are 
# sub-classes of Acquisition, Avoidance, AggressiveCriminalOrHostileAct, 
# FriendlyOrSupportiveAct and Cognition.
# 
# These subclasses should be extended as needed for a domain of interest.
# 
# Created: April 1 2021
# Last Modified: October 31 2023
# 
# Licensed by OntoInsights, LLC
# Creative Commons Attribution 4.0 International (CC BY 4.0)
# 
# Unless required by applicable law or agreed to in writing,
# software distributed under the License is distributed on an
# "AS IS" BASIS, WITHOUT WARRANTIES OR CONDITIONS OF ANY KIND,
# either express or implied.
# 
# Changes:
#  Reset change history and simplified
########################################################################


########################################################################
# Classes
########################################################################

:Abduction a owl:Class ;
  rdfs:subClassOf :CaptureAndSeizure ;
  rdfs:label "Abduction"@en ;
  rdfs:comment "An act of taking an Agent (a Person or GroupOfAgents/Persons) against their will."@en ;
  :wordnet_noun_synset "00776957", "00777199", "00784853" ;
  :wordnet_verb_synset "01473673", "01474455" .

:AidAndAssistance a owl:Class ;
  rdfs:subClassOf :FriendlyOrSupportiveAct ;
  rdfs:label "Aid and Assistance"@en ;
  rdfs:comment "An act that helps someone/something."@en ;
  :wordnet_noun_synset "00656128", "01063127", "01090092", "13286803" ;
  :wordnet_verb_synset "00081834", "02553283" .

:Arson a owl:Class ;
  rdfs:subClassOf :AttackDamageAndAssault ;
  rdfs:label "Arson"@en ;
  rdfs:comment "An Event where a fire is intentionally set in order to destroy or damage property."@en ;
  :wordnet_noun_synset "00378877", "03571171" ;
  :wordnet_verb_synset "00378713" .

:AssessmentAndCharacterization a owl:Class ;
  rdfs:subClassOf :Cognition ;
  rdfs:label "Assessment and Characterization"@en ;
  rdfs:comment "Events dealing with evaluating, characterizing or estimating something or someone."@en ;
  :wordnet_noun_synset "00875745", "05740701", "00143485", "05770995", "05811387" ;
  :wordnet_verb_synset "00672179", "00958719", "00654571", "02170904", "00636134", "01028104", "00594278", "00683348", "00674352" .

:AttackDamageAndAssault a owl:Class ;
  rdfs:subClassOf :AggressiveCriminalOrHostileAct ;
  rdfs:label "Attack, Damage and Assault"@en ;
  rdfs:comment "An aggressive action taken against other Agent(s) and/or things and which is intended to cause harm or damage. If the action involved the use of weapons, these can identified using the :has_instrument property. The location of the attack or damage is defined using the :has_location property, while the attacking Agents are specified using the :has_active_agent predicate. The thing or Agent that is attacked is defined using the :has_affected_resource/:has_affected_agent predicates (respectively). Note that if the action involved a statement/communication, then the Event should also be classified as a :CommunicationAndSpeechAct."@en ;
  :wordnet_noun_synset "00403900", "00974725", "00982124", "00775311", "00217881" ;
  :wordnet_verb_synset "00864347", "00259743", "00090640", "00478872" . 

:AttentionAndFocus a owl:Class ;
  rdfs:subClassOf :Cognition ;
  rdfs:label "Attention and Focus"@en ;
  rdfs:comment "The act of a Person paying attention to/concentrating on something or someone. The entity who/which is concentrated on is indicated by the :has_topic property."@en ;
  :wordnet_noun_synset "05658424", "05712641", "00880604", "05712213", "04670308", "05708052" ;
  :wordnet_verb_synset "00724156", "02134765", "01787213" .

:Battle a owl:Class ;
  rdfs:subClassOf :AttackDamageAndAssault ;
  rdfs:label "Battle"@en ;
  rdfs:comment "Any Event that involves fighting (typically) between military/paramilitary/armed forces."@en ;
  :wordnet_noun_synset "00955670", "00961007" ;
  :wordnet_verb_synset "01092746", "01126191" .

:Belief a owl:Class ;
  rdfs:subClassOf :Cognition ;
  rdfs:label "Belief"@en ;
  rdfs:comment "An 'attitude that something is the case, or that some proposition about the world is true' (https://en.wikipedia.org/w/index.php?title=Belief&oldid=1013662709)."@en ;
  :wordnet_noun_synset "05950141", "05734038" ;
  :wordnet_verb_synset "00685199", "00923043" . 

:Betrayal a owl:Class ;
  rdfs:subClassOf :DeceptionAndDishonesty, :ViolationOfAgreement ;
  rdfs:label "Betrayal"@en ;
  rdfs:comment "From Wikipedia (https://en.wikipedia.org/w/index.php?title=Betrayal&oldid=1096433753), Betrayal 'is the breaking or violation of a presumptive contract, trust, or confidence that produces moral and psychological conflict within a relationship amongst individuals, between organizations or between individuals and organizations. Often betrayal is the act of supporting a rival group, or it is a complete break from previously decided upon or presumed norms by one party from the others.'"@en ;
  :wordnet_noun_synset "00751065" ;
  :wordnet_verb_synset "02582588", "02584093", "02543073" . 

:BoycottAndBan a owl:Class ;
  rdfs:subClassOf :Avoidance, :RefusalAndRejection ;
  rdfs:label "Boycott and Ban"@en ;
  rdfs:comment "An act of abstaining from interacting with (such as working with or buying from) an Agent. The Agent which is boycotting another entity is identified using :has_active_agent, while the Agent boycotted against is specified using :has_affected_agent."@en ;
  :wordnet_noun_synset "00206979", "07269842", "06673141" ;
  :wordnet_verb_synset "02470917", "02509666" .

:CaptureAndSeizure a owl:Class ;
  rdfs:subClassOf :Acquisition, :AggressiveCriminalOrHostileAct, :ChangeOfPossession ;
  rdfs:label "Capture and Seizure"@en ;
  rdfs:comment "An act involved taking possession or control of some Resource or some Agent, by force. The Agent who performs the act is specified using the :has_active_agent property, while the Agent which is taken, controlled, or otherwise affected by the act is identified using :has_affected_agent. If a thing/Resource is captured, that entity is indicated using the :has_topic predicate."@en ;
  :wordnet_noun_synset "00089301", "00097789", "00776783", "00086039" ;
  :wordnet_verb_synset "01217985", "01215136", "01217701", "02210054" .

:CoercionAndIntimidation a owl:Class ;
  rdfs:subClassOf :AggressiveCriminalOrHostileAct ;
  rdfs:label "Coercion and Intimidation"@en ;
  rdfs:comment "An action involving the use of force and/or authority to compel or prevent action, and/or to induce fear."@en ;
  :wordnet_noun_synset "00157632", "01224966", "05202630", "14019785" ; 
  :wordnet_verb_synset "02510211", "01823521", "01037071", "02512195", "02502465" .

:Concealment a owl:Class ;
  rdfs:subClassOf :Prevention ;
  rdfs:label "Concealment"@en ;
  rdfs:comment "An act of preventing something/someone from being known/found."@en ;
  :wordnet_noun_synset "01050836", "04659534", "04254139" ;
  :wordnet_verb_synset "02149298", "02163017", "00314788" . 

:DeceptionAndDishonesty a owl:Class ;
  rdfs:subClassOf :AggressiveCriminalOrHostileAct ;
  rdfs:label "Deception and Dishonesty"@en ;
  rdfs:comment "An act of preventing something/someone from being known/found."@en ;
  :wordnet_noun_synset "00752488", "00750872", "00751748" ;
  :wordnet_verb_synset "02581157",  "02580280", "02583006", "02580591" .

:DecisionMakingAndChoice a owl:Class ;
  rdfs:subClassOf :Cognition ;
  rdfs:label "Decision Making and Choice"@en ;
  rdfs:comment "An act of concluding or resolving some question or issue by choosing a course of action or alternative."@en ;
  :wordnet_noun_synset "00162063", "00039000", "00152317" ;
  :wordnet_verb_synset "02486392", "00681856", "00699355" .

:DefensiveAndProtectiveAct a owl:Class ;
  rdfs:subClassOf :FriendlyOrSupportiveAct ;
  rdfs:label "Defensive and Protective Act"@en ;
  rdfs:comment "An action intended to prevent or lessen harm or damage, or to protect from aggression. If the action involved the use of weapons, these can identified using the :has_instrument property. Note that if the action involved a statement/communication, then the Event should also be classified as a :CommunicationAndSpeechAct."@en ;
  :wordnet_noun_synset "00819341" ;
  :wordnet_noun_synset "01130221", "01130619" .

:EmotionalResponse a owl:Class ;
  rdfs:subClassOf :Cognition ;
  rdfs:label "Emotional Response"@en ;
  rdfs:comment "A state of mind associated with positive/pleasurable or negative/displeasurable feelings, thoughts and moods."@en ;
  :wordnet_noun_synset "00026390", "07495208", "11437243" ;
  :wordnet_verb_synset "00692071", "00719282" .

:EscapeAndEvasion a owl:Class ;
  rdfs:subClassOf :Avoidance, :MovementTravelAndTransportation ;
  rdfs:label "Escape and Evasion"@en ;
  rdfs:comment "An act of avoiding/getting away from something, someone or some Event, or of breaking free from captivity or oppression."@en ;
  :wordnet_noun_synset "00046918", "01247140", "00060196" ;
  :wordnet_verb_synset "00812391", "02078305", "02078906" .

:Exhaustion a owl:Class ;
  rdfs:subClassOf :SensoryPerception ;
  rdfs:label "Exhaustion"@en ;
  rdfs:comment "A feeling of discomfort caused by a lack of sleep, over exertion, etc."@en ;
  :wordnet_noun_synset "14039832", "00634960" ;
  :wordnet_verb_synset "00074774", "00030640" . 

:Forgetting a owl:Class ;
  rdfs:subClassOf :Cognition ;
  rdfs:label "Forgetting"@en ;
  rdfs:comment "An act of Cognition where past occurrences, learning and insights cannot be recalled/remembered."@en ;
  :wordnet_noun_synset "05681752" ;
  :wordnet_verb_synset "00610654", "00611721", "00616520", "00599897", "00600024" .

:GiftAndDonation a owl:Class ;
  rdfs:subClassOf :Acquisition, :FriendlyOrSupportiveAct, :ChangeOfPossession ;
  rdfs:label "Gift and Donation"@en ;
  rdfs:comment "An act of giving with no expectation of payment."@en ;
  :wordnet_noun_synset "01088005", "01091702", "13285910", "13290913" ;
  :wordnet_verb_synset "01062618", "02206050", "02313721", "02204104", "02205200" .

:IgnoringAndOverlooking a owl:Class ;
  rdfs:subClassOf :Avoidance, :Cognition ;
  rdfs:label "Ignoring and Overlooking"@en ;
  rdfs:comment "An act of purposefully disregarding, not noticing or not acknowledging something or someone."@en ;
  :wordnet_noun_synset "00200890", "00419628", "05714175" ; 
  :wordnet_verb_synset "00596900", "00618547", "00802592", "02123706", "01061436", "00616690", "02170805", "00596701" .

:IntentionAndGoal a owl:Class ;
  rdfs:subClassOf :Cognition ;
  rdfs:label "Intention and Goal"@en ;
  rdfs:comment "An event or condition that an Agent hopes to attain/accomplish. Intentions are often distinguished from goals by being focused on the present moment, while goals are focused on the future."@en ;
  :wordnet_noun_synset "00023953", "05989760", "00164054", "05907175", "05991800" ; 
  :wordnet_verb_synset "00710809", "00710367", "00711208", "00706456" .

:InvasionAndOccupation a owl:Class ;
  rdfs:subClassOf :CaptureAndSeizure ;
  rdfs:label "Invasion and Occupation"@en ;
  rdfs:comment "Taking and maintaining control of something/some place (for example, a country) by force. The Agent doing the invading/occupying is identified using the :has_active_agent property, while the entity that is invaded/occupied is specified using :has_affected_agent or :has_resource."@en ;
  :wordnet_noun_synset "00977538", "00079356", "00089847", "01135427" ;
  :wordnet_verb_synset "01128786", "00463047", "02277394", "02308993" .

:KnowledgeAndSkill a owl:Class ;
  rdfs:subClassOf :Cognition, :Resource ;
  rdfs:label "Knowledge and Skill"@en ;
  rdfs:comment "Involved with 'a familiarity, awareness, or understanding of someone or something, such as facts (descriptive knowledge), skills (procedural knowledge), or objects (acquaintance knowledge). By most accounts, knowledge can be acquired in many different ways and from many sources, including but not limited to perception, reason, memory, testimony, scientific inquiry, education, and practice.' (https://en.wikipedia.org/w/index.php?title=Knowledge&oldid=1014835309)"@en ;
  :wordnet_noun_synset "05648278", "04897307", "05629222", "05813910", "05625389", "05160767", "05624569" ;
  :wordnet_verb_synset "00595732", "00596016", "00597025", "00597330", "00597527", "00597879", "00598039", "00590283", "00589616", "00592510" .

:LearningAndEducation a owl:Class ;
  rdfs:subClassOf :Acquisition, :KnowledgeAndSkill ;
  rdfs:label "Learning and Education"@en ;
  rdfs:comment "An act of acquiring or transferring knowledge and skills through study, repetition, experience and instruction. This semantic also includes education-related activities such as graduations and awarding of certificates, test taking, attending classes, etc."@en ;
  :wordnet_noun_synset "05760541", "00729939", "00798247", "00891150", "00895653", "00730147", "00884975", "00637704", "06710094", "06490253" ;
  :wordnet_verb_synset "00600349", "00599310", "00601387", "00608509", "00830768", "02392628", "02268987" .

:MaintenanceAndRepair a owl:Class ;
  rdfs:subClassOf :FriendlyOrSupportiveAct ;
  rdfs:label "Maintenance and Repair"@en ;
  rdfs:comment "Any act that maintains/fixes/mends/adjusts/restores an entity."@en ;
  :wordnet_noun_synset "00249844" ; 
  :wordnet_verb_synset "00261534", "01634614", "00206293", "00207826", "00230988", "01572394" .

:Memory a owl:Class ;
  rdfs:subClassOf :Cognition ;
  rdfs:label "Memory"@en ;
  rdfs:comment "An act of Cognition dealing with the recollection/retrieval of past occurrences, learning and insights."@en ;
  :wordnet_noun_synset "05659244", "05763153", "05768199", "05943778" ;
  :wordnet_verb_synset "00611237", "00609334", "00612810", "00613356" .

:Mistake a owl:Class ;
  rdfs:subClassOf :AssessmentAndCharacterization, :TroubleAndProblem ;
  rdfs:label "Mistake"@en ;
  rdfs:comment "An act of Cognition/judgment indicating that a previous EventAndState (such as an AggressiveCriminalOrHostileAct, decision or Belief) was incorrect, wrong or faulty. The previous EventAndState is identified using the :has_topic property."@en ;
  :wordnet_noun_synset "05714576", "05902260", "04811700" ;
  :wordnet_verb_synset "00641140", "00621541", "00619438" .

:MurderAndHomicide a owl:Class ;
  rdfs:subClassOf :AttackDamageAndAssault, :Death ;
  rdfs:label "Murder and Homicide"@en ;
  rdfs:comment "Any Event that is related to killing a person or living thing."@en ;
  :wordnet_noun_synset "00220890" ;
  :wordnet_verb_synset "01326622" .

:Pain a owl:Class ;
  rdfs:subClassOf :SensoryPerception ;
  rdfs:label "Pain"@en ;
  rdfs:comment "A reaction of suffering or discomfort."@en ;
  :wordnet_noun_synset "05732639", "07509503", "14346126", "07510467" ;
  :wordnet_verb_synset "02125976" . 

:Prevention a owl:Class ;
  rdfs:subClassOf :Avoidance ;
  rdfs:label "Prevention"@en ;
  rdfs:comment "An act of stopping some event or condition from occurring. Note that the event/state/condition is identified using the :has_topic property."@en ;
  :wordnet_noun_synset "01075919" ;
  :wordnet_verb_synset "02455370", "02456941", "02456614", "00772186", "00910052", "02563998" .

:PurchaseAndSale a owl:Class ;
  rdfs:subClassOf :Acquisition, :FinancialEvent, :ChangeOfPossession ;
  rdfs:label "Purchase and Sale"@en ;
  rdfs:comment "An act of Acquisition/transfer of ownership of something by the exchange of money, assets, etc. The 'buyer' is identified using the property, :has_active_agent, while the 'seller' is identified using the :has_affected_agent predicate. The details of what monies, assets, etc. are used are expressed using the :has_instrument property, while the thing sold is defined using the :has_topic property."@en ;
  :wordnet_noun_synset "00084549", "00079838", "00791195", "00079838", "01115160", "10498913" ; 
  :wordnet_verb_synset "02211988", "02262178" .

:Resistance a owl:Class ;
  rdfs:subClassOf :AggressiveCriminalOrHostileAct, :RefusalAndRejection ;
  rdfs:label "Resistance"@en ;
  rdfs:comment "An act of opposition to someone or something, or a refusal to accept or comply with something. The entity that is being resisted is identified using the :has_topic predicate."@en ;
  :wordnet_noun_synset "00203133", "01171807", "00966007", "00964240" ;
  :wordnet_verb_synset "01093838", "02712676", "02590043", "02589224" .

:RobberyAndTheft a owl:Class ;
  rdfs:subClassOf :CaptureAndSeizure ;
  rdfs:label "Robbery and Theft"@en ;
  rdfs:comment "An act involved with taking something unlawfully, from an Agent. The Agent who is the thief is specified using the :has_active_agent property, while the Agent stolen from is identified using :has_affected_agent. The thing(s) taken are indicated using the :has_topic predicate."@en ;
  :wordnet_noun_synset "00782543", "00786699" ;
  :wordnet_verb_synset "02326737" . 

:ScienceAndTechnology a owl:Class ;
  rdfs:subClassOf :KnowledgeAndSkill ;
  rdfs:label "Science and Technology"@en ;
  rdfs:comment "Superclass for various areas of study 'of the structure and behavior of the physical world, especially by watching, measuring, and doing experiments, and the development of theories to describe the results of these activities' (https://dictionary.cambridge.org/us/dictionary/english/science)."@en ;
  :wordnet_noun_synset "06008975", "06005806" .

:SensoryPerception a owl:Class ;
  rdfs:subClassOf :Cognition ;
  rdfs:label "Sensory Perception"@en ;
  rdfs:comment "An act involving one of the senses - sight, hearing, touch, taste and smell."@en ;
  :wordnet_noun_synset "05729937", "05660241" ;
  :wordnet_verb_synset "02129213", "02133754", "02174146", "02174335", "02110460", "02131823", "02168177", "02195992" . 

:SexualAssaultAndRape a owl:Class ;
  rdfs:subClassOf :AttackDamageAndAssault ;
  rdfs:label "Sexual Assault and Rape"@en ;
  rdfs:comment "Any Event that involves sexual assault of a Person."@en ;
  :wordnet_noun_synset "00775604" ;
  :wordnet_verb_synset "02573434" . 

:Supervision a owl:Class ;
  rdfs:subClassOf :AttentionAndFocus ;
  rdfs:label "Supervision"@en ;
  rdfs:comment "The act of a Person paying attention to/overseeing/monitoring someone or something. The entity who/which is supervised is indicated by the :has_topic property."@en ;
  :wordnet_noun_synset "01135602" ;
  :wordnet_verb_synset "02173796", "02436818" .


########################################################################
# Disjointness
########################################################################

[] rdf:type owl:AllDisjointClasses ;
  owl:members  ( :AttackDamageAndAssault :MaintenanceAndRepair ) .

[] rdf:type owl:AllDisjointClasses ;
  owl:members  ( :AttentionAndFocus :IgnoringAndOverlooking ) .

[] rdf:type owl:AllDisjointClasses ;
  owl:members  ( :Forgetting :Memory ) .

[] rdf:type owl:AllDisjointClasses ;
  owl:members  ( :GiftAndDonation :RobberyAndTheft ) .

[] rdf:type owl:AllDisjointClasses ;
  owl:members  ( :MurderAndHomicide :Suicide ) .

