@prefix : <urn:ontoinsights:dna:> .
@prefix dna: <urn:ontoinsights:dna:> .
@prefix owl: <http://www.w3.org/2002/07/owl#> .
@prefix rdf: <http://www.w3.org/1999/02/22-rdf-syntax-ns#> .
@prefix rdfs: <http://www.w3.org/2000/01/rdf-schema#> .
@prefix xsd: <http://www.w3.org/2001/XMLSchema#> .

########################################################################
# File defining general concepts used throughout the DNA ontologies
# 
# Created: February 9 2020
# Last modified: November 6 2023
# 
# Licensed by OntoInsights, LLC
# Creative Commons Attribution 4.0 International (CC BY 4.0)
# 
# Unless required by applicable law or agreed to in writing,
# software distributed under the License is distributed on an
# "AS IS" BASIS, WITHOUT WARRANTIES OR CONDITIONS OF ANY KIND,
# either express or implied.
# 
# Changes:
#  Reset change history and simplified
#  Removed invalid "subclassOf" predicate 
########################################################################


########################################################################
# Annotation Properties
########################################################################

:example a owl:AnnotationProperty ;
  rdfs:label "example"@en ;
  rdfs:comment "Words/text that illustrate the concept/semantic being defined or whose instances would be specified as types of the concept/semantic."@en .

:synonym a owl:AnnotationProperty ;
  rdfs:label "synonym"@en ;
  rdfs:comment "A word which has a similar meaning."@en .

:wordnet_noun_synset a owl:AnnotationProperty ;
  rdfs:label "WordNet noun synset"@en ;
  rdfs:comment "String holding the WordNet synset identifier for the concept. WordNet is described and available from the following web site, https://wordnet.princeton.edu/. Note that there may be more than one synset corresponding to a concept."@en ;
  rdfs:range xsd:string .

:wordnet_verb_synset a owl:AnnotationProperty ;
  rdfs:label "WordNet verb synset"@en ;
  rdfs:comment "String holding the WordNet synset identifier for the concept. WordNet is described and available from the following web site, https://wordnet.princeton.edu/. Note that there may be more than one synset corresponding to a concept."@en ;
  rdfs:range xsd:string .


########################################################################
# Classes
########################################################################

:Agent a owl:Class ;
  rdfs:label "Agent"@en ;
  rdfs:comment "Superclass representing any entity, such as a person, organization or organism, that can influence or be influenced by its environment. Agents are the participants in, are affected by or are the holders of EventAndState occurrences and conditions. Note that an 'imaginary' being/Agent is identified using the :imaginary boolean."@en ;
  :wordnet_noun_synset "00007347", "09786620", "09836176", "09506868" .

:Collection a owl:Class ;
  rdfs:label "Collection"@en ;
  rdfs:comment "A grouping whose members are defined using the :has_member property, or whose members are specifically excluded using the :excluded_member property."@en ;
  :wordnet_noun_synset "01016008" .

:EventAndState a owl:Class ;
  rdfs:label "Event and State"@en ;
  rdfs:comment "Superclass for any occurrence/event, factor or condition/state. An event is an occurrence or happening that is typically described by what happened (the specific subclass of :EventAndState), to whom (defined using :has_agent or its sub-properties), when (defined using :has_time property or its sub-properties), how (defined using :has_instrument) and where (defined using :has_location or its sub-properties). A state is a factor, situation or condition that an Agent (defined using :has_agent or its subproperty, :has_holder) or Resouce (defined using :has_object) experiences at some time (defined using :has_time or its sub-properties) and possibly place (defined using :has_location)."@en ;
  :wordnet_noun_synset "07298313", "00024900", "08584764", "13957629" .

:GoalDirectedProcess a owl:Class ;
  rdfs:label "Goal-Directed Process"@en ;
  rdfs:subClassOf :Process ;
  rdfs:comment "A series of interrelated/interdependent events or states/conditions that progress along a timeline that are specifically designed to achieve a goal (where the goal is indicated using the property, :has_goal)."@en ;
  :wordnet_noun_synset "01025762" . 

:InformationGraph a owl:Class ;
  rdfs:label "Information Graph"@en ;
  rdfs:subClassOf :InformationSource ;
  rdfs:comment "A collection of entities (the 'nodes') representing specific instances of the types of things in a domain of interest, interconnected by named 'edges' which identify the entities' properties (such as string or integer values) and relationships between them. The structure and semantics of the graph ('knowledge') are derived by this (DNA) ontology."@en .

:InformationSource a owl:Class ;
  rdfs:label "Information Source"@en ;
  rdfs:comment "A document, book, news article, database, spreadsheet, file, web page or other textual artifact with non-fictional, or fictional content."@en ;
  :wordnet_noun_synset "06278749", "03222161", "06650349", "06520807", "06413674" .

:Location a owl:Class ;
  rdfs:label "Location"@en ;
  rdfs:comment "A place, whether real, virtual or imagined. Locations can be defined by coordinates (such as latitude and longitude), by name (such as geopolitical entities), by online location (such as an IP address or URL), by geographic or anthropogenic feature (such as the name of a body of water or a road), etc. An Event's or State's Location is specified using the :has_location property or one of its subproperties. Note that an 'imaginary' Location (such as C.S. Lewis' Narnia) is identified using the :imaginary boolean."@en ;
  :wordnet_noun_synset "05633662" . 

:Narrative a owl:Class ;
  rdfs:label "Narrative"@en ;
  rdfs:subClassOf :InformationSource ;
  rdfs:comment "A sequence of events relating/explaining what occurred in a (real or fictitious) world."@en ;
  :wordnet_noun_synset "07235754" .

:NaturalProcess a owl:Class ;
  rdfs:label "Natural Process"@en ;
  rdfs:subClassOf :Process ;
  rdfs:comment "A series of interrelated/interdependent events or states/conditions that progress along a timeline. Examples are the aging process, climate change or a chemical process."@en ;
  :wordnet_noun_synset "00029976" .

:Process a owl:Class ;
  rdfs:label "Process/Sequence"@en ;
  rdfs:comment "A series of interrelated and/or interdependent events or states/conditions that progress along a timeline or that may be specifically designed to achieve a goal. Subclasses are NaturalProcesses (such as the aging process, climate change or a chemical process) or GoalDirectedProcesses (which describes a business process or series of actions that are designed to achieve a specific end state)."@en .

:Quote a owl:Class ;
  rdfs:subClassOf :Sentence ;
  rdfs:label "Quote"@en ;
  rdfs:comment "A statement spoken, written or otherwise communicated by an Agent."@en ;
  :wordnet_noun_synset "01032674" .

:Resource a owl:Class ;
  rdfs:label "Resource"@en ;
  rdfs:comment "Superclass defining any inanimate entity (such as a food, tools, building, ...) which can be used, harvested, mined, made/manufactured, bought and sold. Note that an 'imaginary' Resource (such as a flying carpet or magic wand) is identified using the :imaginary boolean."@en ;
  :wordnet_noun_synset "13352793" .

:Sentence a owl:Class ;
  rdfs:label "Sentence"@en ;
  rdfs:subClassOf :InformationSource ;
  rdfs:comment "A portion of an InformationSource written as unstructured text, ending with a period, question or exclamation mark, etc., typically with one or more subjects, verbs and objects."@en .

:Time a owl:Class ;
  rdfs:label "Time"@en ;
  rdfs:comment "Superclass defining the shared semantics of specific points in time, intervals of time or durations. An individual's time-related information is specified using the :has_time property or its sub-properties."@en ;
  :wordnet_noun_synset "00028468" .


########################################################################
# Datatype Properties
########################################################################

:alternative a owl:DatatypeProperty, owl:FunctionalProperty ;
  rdfs:label "alternative (boolean)"@en ;
  rdfs:comment "Boolean indicating that a Collection holds different 'alternatives'/possibilities. If not specified, :alternatives is assumed to be false."@en ;
  :example "For example, ':alternatives true' is used to describe the Collection of Locations, 'grocery store' and 'Farmers' Market' in the sentence, 'John went to either the grocery store or the Farmers' Market.'"@en ;
  rdfs:domain :Collection ;
  rdfs:range xsd:boolean .

:confidence a owl:DatatypeProperty, owl:FunctionalProperty ;
  rdfs:label "confidence"@en ;
  rdfs:comment "Decimal from 0.0 to 1.0 defining the certainty that the referencing entity or a subject-predicate-object statement is correctly defined defined, based on its InformationSource(s). When used with a subject-predicate-object triple, the property is defined as an RDF* property extension on the predicate."@en ;
  rdfs:range [ a rdfs:Datatype ;
               owl:onDatatype xsd:decimal ;
               owl:withRestrictions ( [ xsd:minInclusive "0.00"^^xsd:decimal ]
                                      [ xsd:maxInclusive "1.00"^^xsd:decimal ] ) ] .

:count a owl:DatatypeProperty ;
  rdfs:label "count/number"@en ;
  rdfs:comment "The number of some entity/in a Collection."@en ;
  :example "For example, for the sentence, 'Three motorcyclists rode down the street.', a Collection (of motorcyclists) would be instantiated with a :count of 3."@en ;
  rdfs:domain :Collection ;
  rdfs:range xsd:integer .

:external_link a owl:DatatypeProperty ;
  rdfs:label "external link"@en ;
  rdfs:comment "Text specifying a URL/URI where more information about the referencing entity can be found."@en ;
  rdfs:range xsd:string .
  
:future a owl:DatatypeProperty, owl:FunctionalProperty ;
  rdfs:label "future (boolean)"@en ;
  rdfs:comment "Boolean indicating that the individual describes somthing possible in, or planned for, a 'future' time."@en ;
  rdfs:range xsd:boolean .
  
:imaginary a owl:DatatypeProperty, owl:FunctionalProperty ;
  rdfs:label "imaginary (boolean)"@en ;
  rdfs:comment "Boolean indicating that the individual describes somthing that exists in the imagination (in stories, myth, etc.) but does not exist in reality."@en ;
  rdfs:range xsd:boolean .

:maximum_count a owl:DatatypeProperty, owl:FunctionalProperty ;
  rdfs:label "maximum count/number"@en ;
  rdfs:comment "The maximum number of some entity when an exact count is not known."@en ;
  :example "For example, for the sentence, 'No more than ten motorcyclists rode down the street.', a Collection (of motorcyclists) would be instantiated with a :maximum_count of 10."@en ;
  rdfs:domain :Collection ;
  rdfs:range xsd:integer .

:minimum_count a owl:DatatypeProperty, owl:FunctionalProperty ;
  rdfs:label "minimum count/number"@en ;
  rdfs:comment "The minimum number of some entity when an exact count is not known."@en ;
  :example "For example, for the sentence, 'At least five motorcyclists rode down the street.', a Collection (of motorcyclists) would be instantiated with a :minimum_count of 5."@en ;
  rdfs:domain :Collection ;
  rdfs:range xsd:integer .

:negation a owl:DatatypeProperty, owl:FunctionalProperty ;
  rdfs:label "negation (boolean)"@en ;
  rdfs:range xsd:boolean ;
  rdfs:comment "Indicates whether the referencing entity does NOT exist, did NOT occur/has NOT happened, etc."@en .

:probability a owl:DatatypeProperty, owl:FunctionalProperty ;
  rdfs:label "probability/likelihood"@en ;
  rdfs:comment "Decimal that is an RDF* property extension indicating the likelihood of the subject being related to the object using the predicate. A variety of objects MAY be related to the subject-predicate pair, where the probabilities for all the pairs should add to 1.0. In order to indicate the likelihood that the subject-predicate relationship is NOT applicable, the object can be defined as owl:Nothing."@en ;
  rdfs:comment "An example of the usage of :probability is to indicate that :Bird :Flies {:probability 0.9} \"true\"^^xsd:boolean and :Bird :Flies {:probability 0.1} \"false\"^^xsd:boolean."@en ;
  rdfs:range [ a rdfs:Datatype ;
               owl:onDatatype xsd:decimal ;
               owl:withRestrictions ( [ xsd:minInclusive "0.00"^^xsd:decimal ]
                                      [ xsd:maxInclusive "1.00"^^xsd:decimal ] ) ] .

:prototypical a owl:DatatypeProperty, owl:FunctionalProperty ;
  rdfs:label "prototypical (boolean)"@en ;
  rdfs:comment "Boolean indicating that the individual describes a 'typical' (and not a specific) instance."@en ;
  rdfs:comment "This concept can also be indicated by using an OWL class as an instance (via OWL2 punning)."@en ;
  rdfs:range xsd:boolean .


########################################################################
# Object Properties
########################################################################

:adjoins a owl:ObjectProperty ;
  rdfs:label "adjoins"@en ;
  rdfs:comment "Indicates that the boundaries of an entity touch/join with another/share a border or boundary."@en .

:causes a owl:ObjectProperty ;
  rdfs:label "causes"@en ;
  rdfs:comment "Relationship between two EventAndState individuals indicating that the subject is assumed to 'cause' (make happen or result in) the object."@en ;
  rdfs:domain :EventAndState ;
  rdfs:range :EventAndState .

:coincides a owl:ObjectProperty ;
  rdfs:label "coincides"@en ;
  rdfs:comment "Indicates that the specified entity exists at the same time/occurs within the same timeframe as the referenced entity."@en .

:enables a owl:ObjectProperty ;
    rdfs:label "enables"@en ;
    rdfs:comment "Relationship between two EventAndState individuals indicating that the subject 'enables'/allows the object (makes it possible or more likely for the object to occur)."@en ;
    rdfs:domain :EventAndState ;
    rdfs:range :EventAndState .

:encodes a owl:ObjectProperty ;
    rdfs:label "encodes"@en ;
    rdfs:comment "Relationship between an InformationGraph and InformationSource indicating that the Graph captures/'encodes' details from the Source."@en ;
    rdfs:domain :InformationGraph ;
    rdfs:range :InformationSource .

:excluded_member a owl:ObjectProperty ;
  rdfs:label "excluded member"@en ;
  rdfs:comment "Defines an entity that is specifically NOT in a grouping/Collection."@en ;
  rdfs:domain :Collection .

:has_aspect a owl:ObjectProperty ;
  rdfs:label "has_aspect"@en ;
  rdfs:comment "Defines a characteristic of the entity and/or further clarifies it."@en .

:has_beginning a owl:ObjectProperty, owl:FunctionalProperty ;
  rdfs:label "has beginning"@en ;
  rdfs:subPropertyOf :has_time ;
  rdfs:range :Time ;
  rdfs:comment "References a Time that is the start of the existence/time frame of some entity, or that is the beginning of an Interval or Duration."@en .

:has_component a owl:ObjectProperty ;
  rdfs:label "has component"@en ;
  rdfs:comment "Defines a whole-part relationship."@en .

:has_end a owl:ObjectProperty, owl:FunctionalProperty ;
  rdfs:label "has end"@en ;
  rdfs:subPropertyOf :has_time ;
  rdfs:range :Time ;
  rdfs:comment "References a point in time that is the end of the existence/time frame of some entity, or that is the end of an Interval or Duration."@en .

:has_first a owl:ObjectProperty ;
  rdfs:label "has first"@en ;
  rdfs:subPropertyOf :has_component ;
  rdfs:domain :Process ;
  rdfs:range :EventAndState ;
  rdfs:comment "References the first individual in a series of interrelated and/or interdependent events or states/conditions. Note that this is NOT a functional property, and more than one EventAndState may initiate a Process. After the first individual, the 'next' is defined using the :has_next property."@en .

:has_goal a owl:ObjectProperty ;
  rdfs:label "has goal"@en ;
  rdfs:domain [ a owl:Class ;
                owl:unionOf ( :EventAndState :Agent ) ] ;
  rdfs:range :EventAndState ;
  rdfs:comment "References the desired end state (such as reduced pollution levels) or event (such as the release of a new document) - i.e., the 'goal' - of an occurrence, process, meeting, agent, etc."@en .

:has_last a owl:ObjectProperty ;
  rdfs:label "has last"@en ;
  rdfs:subPropertyOf :has_component ;
  rdfs:domain :Process ;
  rdfs:range :EventAndState ;
  rdfs:comment "References the last individual in a series of interrelated and/or interdependent events or states/Conditions. Note that this is NOT a functional property, and more than one EventAndState may terminate a Process. The previous individual references the last using the :has_next property."@en .

:has_location a owl:ObjectProperty ;
  rdfs:label "has location"@en ;
  rdfs:range :Location ;
  rdfs:comment "References where an entity is placed/positioned/resides/occurs/etc."@en .

:has_member a owl:ObjectProperty ;
  rdfs:label "has member"@en ;
  rdfs:comment "Defines an entity that is in a (is a member of a) grouping/Collection."@en ;
  rdfs:domain :Collection .

:has_next a owl:ObjectProperty ;
  rdfs:label "has next"@en ;
  rdfs:comment "Defines an entity that follows the subject/referencing entity in time, or that is an evolution of the entity. :has_next is rather generically defined, but is most likely used in process modeling and related to EventAndState."@en .

:has_time a owl:ObjectProperty ;
  rdfs:label "has time"@en ;
  rdfs:comment "A reference to a Time for a entity, occurrence, factor or condition."@en ;
  rdfs:range :Time .

:overlaps a owl:ObjectProperty ;
  rdfs:label "overlaps"@en ;
  rdfs:comment "Indicates that the boundaries of an entity extend over/cover another."@en .

:prevents a owl:ObjectProperty ;
  rdfs:label "prevents"@en ;
  rdfs:comment "Relationship between two EventAndState individuals indicating that the subject 'prevents' the object (decreases the likelihood of the object occurrring)."@en ;
  rdfs:domain :EventAndState ;
  rdfs:range :EventAndState .
